Work on soundness for untyped judgments

mechanization/theories/Core/Soundness/LogicalRelation/Definitions.v
@@ -33,21 +33,20 @@ Notation "'EG' A ∈ R ↘ Sb " := (R Sb A : ((Prop : (Type : Type)) : (Type : T
 
 
 
-Definition neut_glu_typ_pred {P : PtsSig} a s : glu_typ_pred P :=
+Definition neut_glu_typ_pred {P : PtsSig} s a : glu_typ_pred P :=
   fun Γ A => {{ Γ ⊢ A : Sort@s }} /\
-            (* (forall Δ σ A' K, {{ Δ ⊢w σ : Γ }} -> {{ Δ ⊢ A[σ] ≈ A' }} -> {{ Δ ⊢ A[σ] : K }} -> {{ Δ ⊢ A : K }} -> {{ Δ ⊢ A[σ] ≈ A' : K }}) /\ *)
             (forall Δ σ A', {{ Δ ⊢w σ : Γ }} -> {{ Rne a in length Δ ↘ A' }} -> {{ Δ ⊢ A[σ] ≈ A' : Sort@s }}).
-Arguments neut_glu_typ_pred {P} a s Γ A/.
+Arguments neut_glu_typ_pred {P} s a Γ A/.
 
-Variant neut_glu_exp_pred {P : PtsSig} a s : glu_exp_pred P :=
+Variant neut_glu_exp_pred {P : PtsSig} s a : glu_exp_pred P :=
 | mk_neut_glu_exp_pred :
-  `{ {{ Γ ⊢ A ® neut_glu_typ_pred a s }} ->
+  `{ {{ Γ ⊢ A ® neut_glu_typ_pred s a }} ->
      {{ Γ ⊢ M : A }} ->
      {{ Dom m ≈ m ∈ per_bot }} ->
      (forall Δ σ M', {{ Δ ⊢w σ : Γ }} ->
                    {{ Rne m in length Δ ↘ M' }} ->
                    {{ Δ ⊢ M[σ] ≈ M' : A[σ] }}) ->
-     {{ Γ ⊢ M : A ® ⇑ b m ∈ neut_glu_exp_pred a s }} }.
+     {{ Γ ⊢ M : A ® ⇑ b m ∈ neut_glu_exp_pred s a }} }.
 
 
 Variant pi_glu_typ_pred {P : PtsSig} {s1 s2 s3} (r : Ru P s1 s2 s3)
@@ -56,10 +55,9 @@ Variant pi_glu_typ_pred {P : PtsSig} {s1 s2 s3} (r : Ru P s1 s2 s3)
   (IEl : glu_exp_pred P)
   (OP : forall c (equiv_c : {{ Dom c ≈ c ∈ IR }}), glu_typ_pred P) : glu_typ_pred P :=
 | mk_pi_glu_typ_pred :
-  `{ {{ Γ ⊢ A ≈ Π r IT OT }} ->
-     {{ Γ ⊢ IT }} ->
-     {{ Γ , IT ⊢ OT }} ->
-     (* (forall Δ σ A' K, {{ Δ ⊢w σ : Γ }} -> {{ Δ ⊢ A[σ] ≈ A' }} -> {{ Δ ⊢ A[σ] : K }} -> {{ Δ ⊢ A : K }} -> {{ Δ ⊢ A[σ] ≈ A' : K }}) /\ *)
+  `{ {{ Γ ⊢ A ≈ Π r IT OT : Sort@s3 }} ->
+     {{ Γ ⊢ IT : Sort@s1 }} ->
+     {{ Γ , IT ⊢ OT : Sort@s2 }} ->
      (forall Δ σ, {{ Δ ⊢w σ : Γ }} -> {{ Δ ⊢ IT[σ] ® IP }}) ->
      (forall Δ σ M m,
          {{ Δ ⊢w σ : Γ }} ->
@@ -77,10 +75,9 @@ Variant pi_glu_exp_pred {P : PtsSig} {s1 s2 s3} (r : Ru P s1 s2 s3)
 | mk_pi_glu_exp_pred :
   `{ {{ Γ ⊢ M : A }} ->
      {{ Dom m ≈ m ∈ elem_rel }} ->
-     {{ Γ ⊢ A ≈ Π r IT OT }} ->
-     {{ Γ ⊢ IT }} ->
-     {{ Γ , IT ⊢ OT }} ->
-     (* (forall Δ σ A' K, {{ Δ ⊢w σ : Γ }} -> {{ Δ ⊢ A[σ] ≈ A' }} -> {{ Δ ⊢ A[σ] : K }} -> {{ Δ ⊢ A : K }} -> {{ Δ ⊢ A[σ] ≈ A' : K }}) /\ *)
+     {{ Γ ⊢ A ≈ Π r IT OT : Sort@s3 }} ->
+     {{ Γ ⊢ IT : Sort@s1 }} ->
+     {{ Γ , IT ⊢ OT : Sort@s2 }} ->
      (forall Δ σ, {{ Δ ⊢w σ : Γ }} -> {{ Δ ⊢ IT[σ] ® IP }}) ->
      (forall Δ σ N n,
          {{ Δ ⊢w σ : Γ }} ->
@@ -92,11 +89,33 @@ Variant pi_glu_exp_pred {P : PtsSig} {s1 s2 s3} (r : Ru P s1 s2 s3)
 #[export]
 Hint Constructors neut_glu_exp_pred pi_glu_typ_pred pi_glu_exp_pred : mcpts.
 
-Definition sort_glu_typ_pred {P : PtsSig} (pred_P : PredicativeSig P) (s : P) : glu_typ_pred P :=
-  fun Γ A => {{ Γ ⊢ A ≈ Sort@s }}
-            (* (forall Δ σ A' K, {{ Δ ⊢w σ : Γ }} -> {{ Δ ⊢ A[σ] ≈ A' }} -> {{ Δ ⊢ A[σ] : K }} -> {{ Δ ⊢ A : K }} -> {{ Δ ⊢ A[σ] ≈ A' : K }}) *).
-Arguments sort_glu_typ_pred {P} pred_P s Γ A/.
+Definition sort_glu_typ_pred {P : PtsSig} (pred_P : PredicativeSig P) (s1 s2 : P) : glu_typ_pred P :=
+  fun Γ A => {{ Γ ⊢ A ≈ Sort@s1 : Sort@s2 }}.
+Arguments sort_glu_typ_pred {P} pred_P s1 s2 Γ A/.
 Transparent sort_glu_typ_pred.
+
+
+Inductive glu_nat {P} {s} (r : Ru_nat P s) : ctx P -> exp P -> domain P -> Prop :=
+| glu_nat_zero :
+  `{ {{ Γ ⊢ M ≈ zero : ℕ }} ->
+     glu_nat r Γ M d{{{ zero }}} }
+| glu_nat_succ :
+  `{ {{ Γ ⊢ M ≈ succ M' : ℕ }} ->
+     glu_nat r Γ M' m' ->
+     glu_nat r Γ M d{{{ succ m' }}} }
+| glu_nat_neut :
+  `{ per_bot m m ->
+     (forall {Δ σ M'}, {{ Δ ⊢w σ : Γ }} -> {{ Rne m in length Δ ↘ M' }} -> {{ Δ ⊢ M[σ] ≈ M' : ℕ }}) ->
+     glu_nat r Γ M d{{{ ⇑ a m }}} }.
+
+#[export]
+Hint Constructors glu_nat : mcpts.
+
+Definition nat_glu_typ_pred {P : PtsSig} {s} (r : Ru_nat P s) : glu_typ_pred P := fun Γ A => {{ Γ ⊢ A ≈ ℕ : Sort@s }}.
+Arguments nat_glu_typ_pred {P} {s} r Γ A/.
+
+Definition nat_glu_exp_pred {P : PtsSig} {s} (r : Ru_nat P s) : glu_exp_pred P := fun Γ A M m => {{ Γ ⊢ A ® nat_glu_typ_pred r }} /\ glu_nat r Γ M m.
+Arguments nat_glu_exp_pred {P} {s} r Γ A M m/.
 
 
 Section Gluing.
@@ -114,9 +133,7 @@ Section Gluing.
   Definition sort_glu_exp_pred' {s'} (lt_s'_s : pred_rel pred_P s' s) : glu_exp_pred P :=
     fun Γ A M m =>
       {{ Γ ⊢ M : A }} /\
-        {{ Γ ⊢ A ≈ Sort@s' }} /\
-        (* (forall Δ σ A' K, {{ Δ ⊢w σ : Γ }} -> {{ Δ ⊢ A[σ] ≈ A' }} -> {{ Δ ⊢ A[σ] : K }} -> {{ Δ ⊢ A : K }} -> {{ Δ ⊢ A[σ] ≈ A' : K }}) /\ *)
-        (* (forall Δ σ M' B, {{ Δ ⊢w σ : Γ }} -> {{ Δ ⊢ M[σ] ≈ M' }} -> ({{ Δ ⊢ M[σ] : B }} -> {{ Δ ⊢ M[σ] ≈ M' : B }}) /\ ({{ Δ ⊢ M' : B }} -> {{ Δ ⊢ M[σ] ≈ M' : B }})) /\ *)
+        {{ Γ ⊢ A ≈ Sort@s' : Sort@s }} /\
         {{ Γ ⊢ M ® glu_sort_typ_rec lt_s'_s m }}.
 
   #[global]
@@ -127,7 +144,7 @@ Section Gluing.
     `{ forall typ_rel
          el_rel
          (ax_s'_s : Ax P s' s),
-          typ_rel <∙> sort_glu_typ_pred pred_P s' ->
+          typ_rel <∙> sort_glu_typ_pred pred_P s' s ->
           el_rel <∙> sort_glu_exp_pred' (ord_ax pred_P ax_s'_s) ->
           {{ DG Sort@s' ∈ glu_sort_elem_core ↘ typ_rel ↘ el_rel }} }
 
@@ -153,9 +170,15 @@ Section Gluing.
   | glu_sort_elem_core_neut :
     `{ forall typ_rel el_rel,
           {{ Dom b ≈ b ∈ per_bot }} ->
-          typ_rel <∙> neut_glu_typ_pred b ->
-          el_rel <∙> neut_glu_exp_pred b ->
+          typ_rel <∙> neut_glu_typ_pred s b ->
+          el_rel <∙> neut_glu_exp_pred s b ->
           {{ DG ⇑ Sort@s b ∈ glu_sort_elem_core ↘ typ_rel ↘ el_rel }} }
+
+  | glu_sort_elem_core_nat :
+    `{ forall (r : Ru_nat P s) typ_rel el_rel,
+          typ_rel <∙> nat_glu_typ_pred r ->
+          el_rel <∙> nat_glu_exp_pred r ->
+          {{ DG ℕ ∈ glu_sort_elem_core ↘ typ_rel ↘ el_rel }} }
   .
 
 
@@ -165,7 +188,7 @@ Section Gluing.
       (case_sort :
         forall {s'} typ_rel el_rel
           (ax_s'_s : Ax P s' s),
-          typ_rel <∙> sort_glu_typ_pred pred_P s' ->
+          typ_rel <∙> sort_glu_typ_pred pred_P s' s ->
           el_rel <∙> sort_glu_exp_pred' (ord_ax pred_P ax_s'_s) ->
           motive typ_rel el_rel d{{{ Sort@s' }}})
 
@@ -193,14 +216,20 @@ Section Gluing.
         forall {b}
           typ_rel el_rel,
           {{ Dom b ≈ b ∈ per_bot }} ->
-          typ_rel <∙> neut_glu_typ_pred b ->
-          el_rel <∙> neut_glu_exp_pred b ->
-          motive typ_rel el_rel d{{{ ⇑ Sort@s b }}} ).
+          typ_rel <∙> neut_glu_typ_pred s b ->
+          el_rel <∙> neut_glu_exp_pred s b ->
+          motive typ_rel el_rel d{{{ ⇑ Sort@s b }}} )
+
+      (case_nat :
+        forall (r : Ru_nat P s) typ_rel el_rel,
+          typ_rel <∙> nat_glu_typ_pred r ->
+          el_rel <∙> nat_glu_exp_pred r ->
+          motive typ_rel el_rel d{{{ ℕ }}}).
           
   (* Instance Glu_sort_elem_core_def_wf : WellFounded (pred_rel pred_P) := (wf_rel pred_P). *)
 
   #[derive(equations=no, eliminator=no)]
-  Equations glu_sort_elem_core_strong_ind typ_rel exp_rel a (H : glu_sort_elem_core typ_rel exp_rel a) : motive typ_rel exp_rel a:=
+  Equations glu_sort_elem_core_strong_ind typ_rel exp_rel a (H : glu_sort_elem_core typ_rel exp_rel a) : motive typ_rel exp_rel a :=
   | typ_rel, exp_rel, a, (glu_sort_elem_core_sort typ_rel exp_rel ax_s'_s HT HE) => (case_sort typ_rel exp_rel ax_s'_s HT HE);
   | typ_rel, exp_rel, a, (glu_sort_elem_core_pi r in_rel IP IEL OP OEL typ_rel exp_rel elem_rel glu_a Ha glu_B HPi Htyp Hexp) =>
       (case_pi r
@@ -221,7 +250,9 @@ Section Gluing.
          HPi
          Htyp
          Hexp);
-  | typ_rel, exp_rel, a, (glu_sort_elem_core_neut typ_rel exp_rel Hb Htyp Hexp) => (case_neut typ_rel exp_rel Hb Htyp Hexp).
+  | typ_rel, exp_rel, a, (glu_sort_elem_core_neut typ_rel exp_rel Hb Htyp Hexp) => (case_neut typ_rel exp_rel Hb Htyp Hexp)
+  | typ_rel, exp_rel, a, (glu_sort_elem_core_nat r typ_rel exp_rel Htyp Hexp) => (case_nat r typ_rel exp_rel Htyp Hexp)
+  .
 End Gluing.
   
 #[export]
@@ -241,13 +272,11 @@ Definition glu_sort_typ {P} (pred_P : PredicativeSig P) (s : P) (a : domain P) :
   fun Γ A => exists typ_rel exp_rel, {{ DG a ∈ glu_sort_elem pred_P s ↘ typ_rel ↘ exp_rel }} /\ {{ Γ ⊢ A ® typ_rel }}.
 Arguments glu_sort_typ {P} pred_P s a Γ A/.
 
-Definition sort_glu_exp_pred {P} (pred_P : PredicativeSig P) s : glu_exp_pred P :=
+Definition sort_glu_exp_pred {P} (pred_P : PredicativeSig P) s' s : glu_exp_pred P :=
     fun Γ A M m =>
-      {{ Γ ⊢ M : A }} /\ {{ Γ ⊢ A ≈ Sort@s }} /\
-        (* (forall Δ σ A' K, {{ Δ ⊢w σ : Γ }} -> {{ Δ ⊢ A[σ] ≈ A' }} -> {{ Δ ⊢ A[σ] : K }} -> {{ Δ ⊢ A : K }} -> {{ Δ ⊢ A[σ] ≈ A' }}) /\ *)
-        (* (forall Δ σ M' B, {{ Δ ⊢w σ : Γ }} -> {{ Δ ⊢ M[σ] ≈ M' }} -> ({{ Δ ⊢ M[σ] : B }} -> {{ Δ ⊢ M[σ] ≈ M' : B }}) /\ ({{ Δ ⊢ M' : B }} -> {{ Δ ⊢ M[σ] ≈ M' : B }})) /\ *)
-        {{ Γ ⊢ M ® glu_sort_typ pred_P s m }}.
-Arguments sort_glu_exp_pred {P} pred_P s Γ A M m/.
+      {{ Γ ⊢ M : A }} /\ {{ Γ ⊢ A ≈ Sort@s' : Sort@s }} /\
+        {{ Γ ⊢ M ® glu_sort_typ pred_P s' m }}.
+Arguments sort_glu_exp_pred {P} pred_P s' s Γ A M m/.
 
 
 Section GluingInduction.
@@ -264,8 +293,8 @@ Section GluingInduction.
         forall s s'
           (typ_rel : glu_typ_pred P) (exp_rel : glu_exp_pred P) (ax_s'_s : Ax P s' s),
           (forall typ_rel' exp_rel' a, {{ DG a ∈ glu_sort_elem pred_P s' ↘ typ_rel' ↘ exp_rel' }} -> motive s' typ_rel' exp_rel' a) ->
-          typ_rel <∙> sort_glu_typ_pred pred_P s' ->
-          exp_rel <∙> sort_glu_exp_pred pred_P s' ->
+          typ_rel <∙> sort_glu_typ_pred pred_P s' s ->
+          exp_rel <∙> sort_glu_exp_pred pred_P s' s ->
           motive s typ_rel exp_rel d{{{ Sort@s' }}})
 
       (case_pi :
@@ -294,9 +323,15 @@ Section GluingInduction.
           (typ_rel : glu_typ_pred P)
           (exp_rel : glu_exp_pred P),
           {{ Dom b ≈ b ∈ per_bot }} ->
-          typ_rel <∙> neut_glu_typ_pred b ->
-          exp_rel <∙> neut_glu_exp_pred b ->
-          motive s typ_rel exp_rel d{{{ ⇑ Sort@s b }}}).
+          typ_rel <∙> neut_glu_typ_pred s b ->
+          exp_rel <∙> neut_glu_exp_pred s b ->
+          motive s typ_rel exp_rel d{{{ ⇑ Sort@s b }}})
+
+      (case_nat :
+        forall s (r : Ru_nat P s) (typ_rel : glu_typ_pred P) (exp_rel : glu_exp_pred P),
+          typ_rel <∙> nat_glu_typ_pred r ->
+          exp_rel <∙> nat_glu_exp_pred r ->
+          motive s typ_rel exp_rel d{{{ ℕ }}}).
 
   #[local]
   Ltac def_simp := simp glu_sort_elem in *; mauto 3.
@@ -318,6 +353,7 @@ Section GluingInduction.
              HEl')
         _ (* case_pi s *)
         (case_neut s)
+        (case_nat s)
         typ_rel exp_rel a _.
   Next Obligation.
     eapply ord_ax; eassumption.
@@ -378,14 +414,14 @@ End GluingInduction.
 
 
 
-Inductive glu_typ_unsorted_elem {P} (pred_P : PredicativeSig P) : glu_typ_pred P -> glu_exp_pred P -> domain P -> Prop :=
-| glu_typ_unsorted_sort :
-  `( typ_rel <∙> sort_glu_typ_pred pred_P s ->
-     exp_rel <∙> sort_glu_exp_pred pred_P s ->
-     {{ DG Sort@s ∈ glu_typ_unsorted_elem pred_P ↘ typ_rel ↘ exp_rel }} )
-| glu_typ_unsorted_type :
-  `( {{ DG a ∈ glu_sort_elem pred_P s ↘ typ_rel ↘ exp_rel }} ->
-     {{ DG a ∈ glu_typ_unsorted_elem pred_P ↘ typ_rel ↘ exp_rel }} ).
+(* Inductive glu_typ_unsorted_elem {P} (pred_P : PredicativeSig P) : glu_typ_pred P -> glu_exp_pred P -> domain P -> Prop := *)
+(* | glu_typ_unsorted_sort : *)
+(*   `( typ_rel <∙> sort_glu_typ_pred pred_P s -> *)
+(*      exp_rel <∙> sort_glu_exp_pred pred_P s -> *)
+(*      {{ DG Sort@s ∈ glu_typ_unsorted_elem pred_P ↘ typ_rel ↘ exp_rel }} ) *)
+(* | glu_typ_unsorted_type : *)
+(*   `( {{ DG a ∈ glu_sort_elem pred_P s ↘ typ_rel ↘ exp_rel }} -> *)
+(*      {{ DG a ∈ glu_typ_unsorted_elem pred_P ↘ typ_rel ↘ exp_rel }} ). *)
 
 
 
@@ -406,17 +442,17 @@ Variant glu_elem_bot {P} (pred_P : PredicativeSig P) s a Γ A M m : Prop :=
 Hint Constructors glu_elem_bot : mcpts.
 
 
-Variant glu_elem_bot_unsorted {P} (pred_P : PredicativeSig P) a Γ A M m : Prop :=
-  | glu_elem_bot_unsorted_make : forall typ_rel exp_rel,
-      {{ Γ ⊢ M : A }} ->
-      {{ DG a ∈ glu_typ_unsorted_elem pred_P ↘ typ_rel ↘ exp_rel }} ->
-      {{ Γ ⊢ A ® typ_rel }} ->
-      {{ Dom m ≈ m ∈ per_bot }} ->
-      (forall Δ σ M', {{ Δ ⊢w σ : Γ }} -> {{ Rne m in length Δ ↘ M' }} -> {{ Δ ⊢ M[σ] ≈ M' : A[σ] }}) ->
-      {{ Γ ⊢ M : A ® m ∈ glu_elem_bot_unsorted pred_P a }}.
+(* Variant glu_elem_bot_unsorted {P} (pred_P : PredicativeSig P) a Γ A M m : Prop := *)
+(*   | glu_elem_bot_unsorted_make : forall typ_rel exp_rel, *)
+(*       {{ Γ ⊢ M : A }} -> *)
+(*       {{ DG a ∈ glu_typ_unsorted_elem pred_P ↘ typ_rel ↘ exp_rel }} -> *)
+(*       {{ Γ ⊢ A ® typ_rel }} -> *)
+(*       {{ Dom m ≈ m ∈ per_bot }} -> *)
+(*       (forall Δ σ M', {{ Δ ⊢w σ : Γ }} -> {{ Rne m in length Δ ↘ M' }} -> {{ Δ ⊢ M[σ] ≈ M' : A[σ] }}) -> *)
+(*       {{ Γ ⊢ M : A ® m ∈ glu_elem_bot_unsorted pred_P a }}. *)
 
-#[export]
-Hint Constructors glu_elem_bot_unsorted : mcpts.
+(* #[export] *)
+(* Hint Constructors glu_elem_bot_unsorted : mcpts. *)
 
 
 Variant glu_elem_top {P} (pred_P : PredicativeSig P) s a Γ A M m : Prop :=
@@ -431,16 +467,16 @@ Variant glu_elem_top {P} (pred_P : PredicativeSig P) s a Γ A M m : Prop :=
 Hint Constructors glu_elem_top : mcpts.
 
 
-Variant glu_elem_top_unsorted {P} (pred_P : PredicativeSig P) a Γ A M m : Prop :=
-| glu_elem_top_unsorted_make : forall P El,
-    {{ Γ ⊢ M : A }} ->
-    {{ DG a ∈ glu_typ_unsorted_elem pred_P ↘ P ↘ El }} ->
-    {{ Γ ⊢ A ® P }} ->
-    {{ Dom ⇓ a m ≈ ⇓ a m ∈ per_top }} ->
-    (forall Δ σ w, {{ Δ ⊢w σ : Γ }} -> {{ Rnf ⇓ a m in length Δ ↘ w }} -> {{ Δ ⊢ M[σ] ≈ w : A[σ] }}) ->
-    {{ Γ ⊢ M : A ® m ∈ glu_elem_top_unsorted pred_P a }}.
-#[export]
-Hint Constructors glu_elem_top_unsorted : mcpts.
+(* Variant glu_elem_top_unsorted {P} (pred_P : PredicativeSig P) a Γ A M m : Prop := *)
+(* | glu_elem_top_unsorted_make : forall P El, *)
+(*     {{ Γ ⊢ M : A }} -> *)
+(*     {{ DG a ∈ glu_typ_unsorted_elem pred_P ↘ P ↘ El }} -> *)
+(*     {{ Γ ⊢ A ® P }} -> *)
+(*     {{ Dom ⇓ a m ≈ ⇓ a m ∈ per_top }} -> *)
+(*     (forall Δ σ w, {{ Δ ⊢w σ : Γ }} -> {{ Rnf ⇓ a m in length Δ ↘ w }} -> {{ Δ ⊢ M[σ] ≈ w : A[σ] }}) -> *)
+(*     {{ Γ ⊢ M : A ® m ∈ glu_elem_top_unsorted pred_P a }}. *)
+(* #[export] *)
+(* Hint Constructors glu_elem_top_unsorted : mcpts. *)
 
 
 Variant glu_typ_top {P} (pred_P : PredicativeSig P) (s : P) a Γ A : Prop :=
@@ -453,14 +489,14 @@ Variant glu_typ_top {P} (pred_P : PredicativeSig P) (s : P) a Γ A : Prop :=
 Hint Constructors glu_typ_top : mcpts.
 
 
-Variant glu_typ_top_unsorted {P} (pred_P : PredicativeSig P) (a : domain P) Γ A : Prop :=
-| glu_typ_top_unsorted_make :
-    {{ Γ ⊢ A }} ->
-    {{ Dom a ≈ a ∈ per_top_typ }} ->
-    (forall Δ σ A', {{ Δ ⊢w σ : Γ }} -> {{ Rtyp a in length Δ ↘ A' }} -> {{ Δ ⊢ A[σ] ≈ A' }}) ->
-    {{ Γ ⊢ A ® glu_typ_top_unsorted pred_P a }}.
-#[export]
-Hint Constructors glu_typ_top_unsorted : mcpts.
+(* Variant glu_typ_top_unsorted {P} (pred_P : PredicativeSig P) (a : domain P) Γ A : Prop := *)
+(* | glu_typ_top_unsorted_make : *)
+(*     {{ Γ ⊢ A }} -> *)
+(*     {{ Dom a ≈ a ∈ per_top_typ }} -> *)
+(*     (forall Δ σ A', {{ Δ ⊢w σ : Γ }} -> {{ Rtyp a in length Δ ↘ A' }} -> {{ Δ ⊢ A[σ] ≈ A' }}) -> *)
+(*     {{ Γ ⊢ A ® glu_typ_top_unsorted pred_P a }}. *)
+(* #[export] *)
+(* Hint Constructors glu_typ_top_unsorted : mcpts. *)
 
 
 Variant glu_rel_typ_with_sub {P} (pred_P : PredicativeSig P) (s : P) Δ A σ ρ : Prop :=
@@ -471,13 +507,13 @@ Variant glu_rel_typ_with_sub {P} (pred_P : PredicativeSig P) (s : P) Δ A σ ρ 
         {{ Δ ⊢ A[σ] ® P }} ->
         glu_rel_typ_with_sub pred_P s Δ A σ ρ }.
 
-Variant glu_rel_typ_with_sub_unsorted {P} (pred_P : PredicativeSig P) Δ A σ ρ : Prop :=
-| mk_glu_rel_typ_with_sub_unsorted :
-  `{ forall typ_rel exp_rel,
-        {{ ⟦ A ⟧ ρ ↘ a }} ->
-        {{ DG a ∈ glu_typ_unsorted_elem pred_P ↘ typ_rel ↘ exp_rel }} ->
-        {{ Δ ⊢ A[σ] ® typ_rel }} ->
-        glu_rel_typ_with_sub_unsorted pred_P Δ A σ ρ }.
+(* Variant glu_rel_typ_with_sub_unsorted {P} (pred_P : PredicativeSig P) Δ A σ ρ : Prop := *)
+(* | mk_glu_rel_typ_with_sub_unsorted : *)
+(*   `{ forall typ_rel exp_rel, *)
+(*         {{ ⟦ A ⟧ ρ ↘ a }} -> *)
+(*         {{ DG a ∈ glu_typ_unsorted_elem pred_P ↘ typ_rel ↘ exp_rel }} -> *)
+(*         {{ Δ ⊢ A[σ] ® typ_rel }} -> *)
+(*         glu_rel_typ_with_sub_unsorted pred_P Δ A σ ρ }. *)
 
 
 (** Gluing model for contexts and substitutions *)
@@ -488,19 +524,19 @@ Arguments nil_glu_sub_pred {P} Δ σ ρ/.
 
 (** The parameters are ordered differently from the Agda version
     so that we can return [glu_sub_pred]. *)
-Variant cons_glu_sub_pred {P} (pred_P : PredicativeSig P) Γ A (TSb : glu_sub_pred P) : glu_sub_pred P :=
+Variant cons_glu_sub_pred {P} (pred_P : PredicativeSig P) (s : P) Γ A (TSb : glu_sub_pred P) : glu_sub_pred P :=
 | mk_cons_glu_sub_pred :
   `{ forall P El,
         {{ Δ ⊢s σ : Γ, A }} ->
         {{ ⟦ A ⟧ ρ ↯ ↘ a }} ->
-        {{ DG a ∈ glu_typ_unsorted_elem pred_P ↘ P ↘ El }} ->
+        {{ DG a ∈ glu_sort_elem pred_P s ↘ P ↘ El }} ->
         {{ #| ρ[0] |↘ m }} ->
         (** Here we use [{{{ A[Wk][σ] }}}] instead of [{{{ A[Wk∘σ] }}}]
             as syntactic judgement derived from that is
             a more direct consequence of [{{ Γ, A ⊢ #0 : A[Wk] }}] *)
         {{ Δ ⊢ #0[σ] : A[Wk][σ] ® m ∈ El }} ->
         {{ Δ ⊢s Wk ∘ σ ® ρ ↯ ∈ TSb }} ->
-        {{ Δ ⊢s σ ® ρ ∈ cons_glu_sub_pred pred_P Γ A TSb }} }.
+        {{ Δ ⊢s σ ® ρ ∈ cons_glu_sub_pred pred_P s Γ A TSb }} }.
 
 (* Variant cons_glu_sub_pred_unsorted {P} (pred_P : PredicativeSig P) Γ A (TSb : glu_sub_pred P) : glu_sub_pred P := *)
 (* | mk_cons_glu_sub_pred_unsorted : *)
@@ -527,11 +563,11 @@ Inductive glu_ctx_env {P} (pred_P : PredicativeSig P) : glu_sub_pred P -> ctx P 
 | glu_ctx_env_cons :
   `{ forall TSb Sb,
         {{ EG Γ ∈ glu_ctx_env pred_P ↘ TSb }} ->
-        {{ Γ ⊢ A }} ->
+        {{ Γ ⊢ A : Sort@s }} ->
         (forall Δ σ ρ,
             {{ Δ ⊢s σ ® ρ ∈ TSb }} ->
-            glu_rel_typ_with_sub_unsorted pred_P Δ A σ ρ) ->
-        Sb <∙> cons_glu_sub_pred pred_P Γ A TSb ->
+            glu_rel_typ_with_sub pred_P s Δ A σ ρ) ->
+        Sb <∙> cons_glu_sub_pred pred_P s Γ A TSb ->
         {{ EG Γ, A ∈ glu_ctx_env pred_P ↘ Sb }} }.
 
 (* Inductive glu_ctx_env_unsorted {P} (pred_P : PredicativeSig P) : glu_sub_pred P -> ctx P -> Prop := *)
@@ -560,14 +596,14 @@ Variant glu_rel_exp_with_sub {P} (pred_P : PredicativeSig P) s Δ M A σ ρ : Pr
         {{ Δ ⊢ M[σ] : A[σ] ® m ∈ El }} ->
         glu_rel_exp_with_sub pred_P s Δ M A σ ρ }.
 
-Variant glu_rel_exp_with_sub_unsorted {P} (pred_P : PredicativeSig P) Δ M A σ ρ : Prop :=
-| mk_glu_rel_exp_with_sub_unsorted :
-  `{ forall typ_rel exp_rel,
-        {{ ⟦ A ⟧ ρ ↘ a }} ->
-        {{ ⟦ M ⟧ ρ ↘ m }} ->
-        {{ DG a ∈ glu_typ_unsorted_elem pred_P ↘ typ_rel ↘ exp_rel }} ->
-        {{ Δ ⊢ M[σ] : A[σ] ® m ∈ exp_rel }} ->
-        glu_rel_exp_with_sub_unsorted pred_P Δ M A σ ρ }.
+(* Variant glu_rel_exp_with_sub_unsorted {P} (pred_P : PredicativeSig P) Δ M A σ ρ : Prop := *)
+(* | mk_glu_rel_exp_with_sub_unsorted : *)
+(*   `{ forall typ_rel exp_rel, *)
+(*         {{ ⟦ A ⟧ ρ ↘ a }} -> *)
+(*         {{ ⟦ M ⟧ ρ ↘ m }} -> *)
+(*         {{ DG a ∈ glu_typ_unsorted_elem pred_P ↘ typ_rel ↘ exp_rel }} -> *)
+(*         {{ Δ ⊢ M[σ] : A[σ] ® m ∈ exp_rel }} -> *)
+(*         glu_rel_exp_with_sub_unsorted pred_P Δ M A σ ρ }. *)
 
 
 Variant glu_rel_sub_with_sub {P} (pred_P : PredicativeSig P) Δ τ (Sb : glu_sub_pred P) σ ρ : Prop :=
@@ -591,11 +627,11 @@ Definition glu_rel_exp_resp_sub_env {P} (pred_P : PredicativeSig P) s Sb M A :=
 Arguments glu_rel_exp_resp_sub_env {P} pred_P s Sb M A/.
 
 
-Definition glu_rel_exp_resp_sub_env_unsorted {P} (pred_P : PredicativeSig P) Sb M A :=
-  forall Δ σ ρ,
-    {{ Δ ⊢s σ ® ρ ∈ Sb }} ->
-    glu_rel_exp_with_sub_unsorted pred_P Δ M A σ ρ.
-Arguments glu_rel_exp_resp_sub_env_unsorted {P} pred_P Sb M A/.
+(* Definition glu_rel_exp_resp_sub_env_unsorted {P} (pred_P : PredicativeSig P) Sb M A := *)
+(*   forall Δ σ ρ, *)
+(*     {{ Δ ⊢s σ ® ρ ∈ Sb }} -> *)
+(*     glu_rel_exp_with_sub_unsorted pred_P Δ M A σ ρ. *)
+(* Arguments glu_rel_exp_resp_sub_env_unsorted {P} pred_P Sb M A/. *)
 
 
 Definition glu_rel_exp {P} (pred_P : PredicativeSig P) Γ M A : Prop :=
@@ -607,20 +643,20 @@ Definition glu_rel_exp {P} (pred_P : PredicativeSig P) Γ M A : Prop :=
         glu_rel_exp_with_sub pred_P s Δ M A σ ρ.
 Arguments glu_rel_exp {P} pred_P Γ M A/.
 
-Definition glu_rel_exp_unsorted {P} (pred_P : PredicativeSig P) Γ M A : Prop :=
-  exists Sb,
-    {{ EG Γ ∈ glu_ctx_env pred_P ↘ Sb }} /\
-      forall Δ σ ρ,
-        {{ Δ ⊢s σ ® ρ ∈ Sb }} ->
-        glu_rel_exp_with_sub_unsorted pred_P Δ M A σ ρ.
-Arguments glu_rel_exp_unsorted {P} pred_P Γ M A/.
+(* Definition glu_rel_exp_unsorted {P} (pred_P : PredicativeSig P) Γ M A : Prop := *)
+(*   exists Sb, *)
+(*     {{ EG Γ ∈ glu_ctx_env pred_P ↘ Sb }} /\ *)
+(*       forall Δ σ ρ, *)
+(*         {{ Δ ⊢s σ ® ρ ∈ Sb }} -> *)
+(*         glu_rel_exp_with_sub_unsorted pred_P Δ M A σ ρ. *)
+(* Arguments glu_rel_exp_unsorted {P} pred_P Γ M A/. *)
 
-Definition glu_rel_typ_unsorted {P} (pred_P : PredicativeSig P) Γ A : Prop :=
-  exists Sb,
-    {{ EG Γ ∈ glu_ctx_env pred_P ↘ Sb }} /\
-      forall Δ σ ρ,
-        {{ Δ ⊢s σ ® ρ ∈ Sb }} ->
-        glu_rel_typ_with_sub_unsorted pred_P Δ A σ ρ.
+(* Definition glu_rel_typ_unsorted {P} (pred_P : PredicativeSig P) Γ A : Prop := *)
+(*   exists Sb, *)
+(*     {{ EG Γ ∈ glu_ctx_env pred_P ↘ Sb }} /\ *)
+(*       forall Δ σ ρ, *)
+(*         {{ Δ ⊢s σ ® ρ ∈ Sb }} -> *)
+(*         glu_rel_typ_with_sub_unsorted pred_P Δ A σ ρ. *)
 
 Definition glu_rel_sub_resp_sub_env {P} (pred_P : PredicativeSig P) Sb Sb' τ :=
   forall Δ σ ρ,
@@ -638,14 +674,14 @@ Definition glu_rel_sub {P} (pred_P : PredicativeSig P) Γ τ Γ' : Prop :=
 Arguments glu_rel_sub {P} pred_P Γ τ Γ'/.
 
 
-Definition glu_rel_sub_unsorted {P} (pred_P : PredicativeSig P) Γ τ Γ' : Prop :=
-  exists Sb Sb',
-    {{ EG Γ ∈ glu_ctx_env pred_P ↘ Sb }} /\
-    {{ EG Γ' ∈ glu_ctx_env pred_P ↘ Sb' }} /\
-      forall Δ σ ρ,
-        {{ Δ ⊢s σ ® ρ ∈ Sb }} ->
-        glu_rel_sub_with_sub pred_P Δ τ Sb' σ ρ.
-Arguments glu_rel_sub {P} pred_P Γ τ Γ'/.
+(* Definition glu_rel_sub_unsorted {P} (pred_P : PredicativeSig P) Γ τ Γ' : Prop := *)
+(*   exists Sb Sb', *)
+(*     {{ EG Γ ∈ glu_ctx_env pred_P ↘ Sb }} /\ *)
+(*     {{ EG Γ' ∈ glu_ctx_env pred_P ↘ Sb' }} /\ *)
+(*       forall Δ σ ρ, *)
+(*         {{ Δ ⊢s σ ® ρ ∈ Sb }} -> *)
+(*         glu_rel_sub_with_sub pred_P Δ τ Sb' σ ρ. *)
+(* Arguments glu_rel_sub {P} pred_P Γ τ Γ'/. *)
 
 
 Notation "⟪ pred_P ⟫ ⊩ Γ" := (glu_rel_ctx pred_P Γ) (in custom judg at level 80, pred_P constr at level 0, Γ custom exp).
@@ -653,6 +689,6 @@ Notation "⟪ pred_P ⟫ Γ ⊩ M : A" := (glu_rel_exp pred_P Γ M A) (in custom
 Notation "⟪ pred_P ⟫ Γ ⊩s τ : Γ'" := (glu_rel_sub pred_P Γ τ Γ') (in custom judg at level 80, pred_P constr at level 0, Γ custom exp, τ custom exp, Γ' custom exp).
 
 (* Notation "⟪ pred_P ⟫ ⊩u Γ" := (glu_rel_ctx_unsorted pred_P Γ) (in custom judg at level 80, pred_P constr at level 0, Γ custom exp). *)
-Notation "⟪ pred_P ⟫ Γ ⊩u M : A" := (glu_rel_exp_unsorted pred_P Γ M A) (in custom judg at level 80, pred_P constr at level 0, Γ custom exp, M custom exp, A custom exp).
-Notation "⟪ pred_P ⟫ Γ ⊩u A" := (glu_rel_typ_unsorted pred_P Γ A) (in custom judg at level 80, pred_P constr at level 0, Γ custom exp, A custom exp).
-Notation "⟪ pred_P ⟫ Γ ⊩su τ : Γ'" := (glu_rel_sub_unsorted pred_P Γ τ Γ') (in custom judg at level 80, pred_P constr at level 0, Γ custom exp, τ custom exp, Γ' custom exp).
+(* Notation "⟪ pred_P ⟫ Γ ⊩u M : A" := (glu_rel_exp_unsorted pred_P Γ M A) (in custom judg at level 80, pred_P constr at level 0, Γ custom exp, M custom exp, A custom exp). *)
+(* Notation "⟪ pred_P ⟫ Γ ⊩u A" := (glu_rel_typ_unsorted pred_P Γ A) (in custom judg at level 80, pred_P constr at level 0, Γ custom exp, A custom exp). *)
+(* Notation "⟪ pred_P ⟫ Γ ⊩su τ : Γ'" := (glu_rel_sub_unsorted pred_P Γ τ Γ') (in custom judg at level 80, pred_P constr at level 0, Γ custom exp, τ custom exp, Γ' custom exp). *)
