mechanization/theories/Core/Soundness/LogicalRelation/CoreLemmas.v
@@ -6,6 +6,103 @@ From McPTS.Core.Soundness.LogicalRelation Require Import CoreTactics Definitions
 From McPTS.Core.Soundness.Weakening Require Export Lemmas.
 Import Domain_Notations.
 
+Lemma glu_nat_per_nat {P} {s} (r : Ru_nat P s) : forall (Γ : ctx P) M a,
+    glu_nat r Γ M a ->
+    {{ Dom a ≈ a ∈ per_nat }}.
+Proof.
+  induction 1; mauto.
+Qed.
+
+#[local]
+Hint Resolve glu_nat_per_nat : mcpts.
+
+Lemma glu_nat_escape {P} {s} (r : Ru_nat P s) : forall (Γ : ctx P) M a,
+    glu_nat r Γ M a ->
+    {{ ⊢ Γ }} ->
+    {{ Γ ⊢ M : ℕ }}.
+Proof.
+  induction 1; intros;
+    try match goal with
+    | H : _ |- _ => solve [gen_presup H; mauto]
+    end.
+  assert {{ Γ ⊢w Id : Γ }} by mauto.
+  match_by_head (per_bot m m) ltac:(fun H => specialize (H (length Γ)) as [M' []]).
+  clear_dups.
+  assert {{ Γ ⊢ M[Id] ≈ M' : ℕ }} by mauto.
+  gen_presups.
+  mauto.
+Qed.
+
+#[export]
+Hint Resolve glu_nat_escape : mcpts.
+
+Lemma glu_nat_resp_ctx_eq {P} {s} (r : Ru_nat P s) : forall (Γ : ctx P) M a Δ,
+    glu_nat r Γ M a ->
+    {{ ⊢ Γ ≈ Δ }} ->
+    glu_nat r Δ M a.
+Proof.
+  induction 1; intros; mauto.
+Qed.
+
+#[local]
+Hint Resolve glu_nat_resp_ctx_eq : mcpts.
+
+Add Parametric Morphism {P} {s} (r : Ru_nat P s) : (glu_nat r)
+    with signature wf_ctx_eq ==> eq ==> eq ==> iff as glu_ctx_env_sub_morphism_iff1.
+Proof.
+  split; mauto using glu_nat_resp_ctx_eq.
+Qed.
+
+Lemma glu_nat_resp_exp_eq {P} {s} (r : Ru_nat P s) : forall (Γ : ctx P) M a,
+    glu_nat r Γ M a ->
+    forall M',
+    {{ Γ ⊢ M ≈ M' : ℕ }} ->
+    glu_nat r Γ M' a.
+Proof.
+  induction 1; intros; mauto 4.
+  econstructor; trivial.
+  intros.
+  transitivity {{{ M[σ] }}}; mauto 2.
+  symmetry.
+  assert {{ Δ ⊢s σ : Γ }} by mauto 2.
+  assert {{ Δ ⊢ M[σ] ≈ M'[σ] : ℕ[σ] }} by mauto 3.
+  mauto.
+Qed.
+
+#[local]
+Hint Resolve glu_nat_resp_exp_eq : mcpts.
+
+Add Parametric Morphism {P} {s} (r : Ru_nat P s) Γ : (glu_nat r Γ)
+    with signature wf_exp_eq Γ {{{ ℕ }}} ==> eq ==> iff as glu_ctx_env_sub_morphism_iff2.
+Proof.
+  split; mauto using glu_nat_resp_exp_eq.
+Qed.
+
+Lemma glu_nat_readback {P} {s} (r : Ru_nat P s) : forall Γ M a,
+    glu_nat r Γ M a ->
+    forall Δ σ M',
+      {{ Δ ⊢w σ : Γ }} ->
+      {{ Rnf ⇓ ℕ a in length Δ ↘ M' }} ->
+      {{ Δ ⊢ M[σ] ≈ M' : ℕ }}.
+Proof.
+  induction 1; intros; progressive_inversion; gen_presups.
+  - transitivity {{{ zero[σ] }}}; mauto 4.
+  - assert {{ Δ ⊢ M'[σ] ≈ M0 : ℕ }} by mauto 4.
+    transitivity {{{ (succ M')[σ] }}}; mauto 3.
+    transitivity {{{ succ M'[σ] }}}; mauto 4.
+  - mauto 4.
+Qed.
+
+Lemma glu_nat_rule_irrelevance {P} {s} (r : Ru_nat P s) : forall Γ M a,
+    glu_nat r Γ M a ->
+    forall (r' : Ru_nat P s), glu_nat r' Γ M a.
+Proof.
+  intros.
+  induction H; mauto 2.
+Qed.
+
+#[local]
+Hint Resolve glu_nat_rule_irrelevance : mcpts.
 
 #[global]
 Ltac simpl_glu_rel :=
@@ -34,18 +131,18 @@ Lemma glu_sort_elem_sort_lvl {P} (pred_P : PredicativeSig P) : forall s typ_rel 
     {{ DG a ∈ glu_sort_elem pred_P s ↘ typ_rel ↘ exp_rel }} ->
     forall Γ A,
       {{ Γ ⊢ A ® typ_rel }} ->
-      {{ Γ ⊢ A }}.
+      {{ Γ ⊢ A : Sort@s }}.
 Proof.
   simpl.
   induction 1 using glu_sort_elem_ind;
     intros; simpl_glu_rel; mauto 2.
 Qed.
 
-Lemma glu_sort_elem_typ_resp_typ_eq {P} (pred_P : PredicativeSig P) : forall s typ_rel exp_rel a,
+Lemma glu_sort_elem_typ_resp_exp_eq {P} (pred_P : PredicativeSig P) : forall s typ_rel exp_rel a,
     {{ DG a ∈ glu_sort_elem pred_P s ↘ typ_rel ↘ exp_rel }} ->
     forall Γ A A',
       {{ Γ ⊢ A ® typ_rel }} ->
-      {{ Γ ⊢ A ≈ A' }} ->
+      {{ Γ ⊢ A ≈ A' : Sort@s }} ->
       {{ Γ ⊢ A' ® typ_rel }}.
 Proof.
   simpl.
@@ -54,217 +151,80 @@ Proof.
   split; [eassumption | ].
   intros.
   transitivity {{{ A[σ] }}}; mauto 4.
-  
-  (* - assert {{ Γ ⊢ A : Sort@s }}. *)
-  (*   { *)
-  (*     assert {{ Γ ⊢ Sort@s' : Sort@s }} by mauto 2. *)
-  (*     assert {{ Γ ⊢ A[Id] ≈ Sort@s' : Sort@s }} by (eapply H4; mauto 3). *)
-  (*     gen_presup H6. *)
-  (*     mauto 2. *)
-  (*   } *)
-  (*   repeat split. *)
-  (*   + etransitivity; mauto 3.       *)
-  (*   + intros. *)
-  (*     assert {{ Δ ⊢ A[σ] ≈ A'[σ] }} by mauto 3. *)
-  (*     assert {{ Δ ⊢ A[σ] ≈ A'[σ] : K }} by (eapply H4; mauto 3). *)
-  (*     assert {{ Δ ⊢ A[σ] ≈ A'0 }} by (etransitivity; mauto 2). *)
-  (*     gen_presup H10. *)
-  (*     assert ({{ Δ ⊢ A[σ] : K }} -> {{ Δ ⊢ A[σ] ≈ A'0 : K }}) by (eapply H4; mauto 4). *)
-  (*     assert {{ Δ ⊢ A[σ] ≈ A'0 : K }} by mauto 2. *)
-  (*     etransitivity; mauto 3. *)
-  (*   + intros. *)
-  (*     assert {{ Δ ⊢ A[σ] ≈ A'[σ] }} by mauto 3. *)
-  (*     assert {{ Δ ⊢ A[σ] ≈ A'0 }} by (etransitivity; mauto 2). *)
-  (*     assert {{ Δ ⊢ A[σ] ≈ A'0 : K }} by (eapply H4; mauto 4). *)
-  (*     gen_presup H11. *)
-  (*     assert ({{ Δ ⊢ A[σ] : K }} -> {{ Δ ⊢ A[σ] ≈ A'[σ] : K }}) by (eapply H4; mauto 4). *)
-  (*     assert {{ Δ ⊢ A[σ] ≈ A'[σ] : K }} by mauto 2. *)
-  (*     etransitivity; mauto 2. *)
-      
-  (* - econstructor; mauto 2. *)
-  (*   + assert {{ Γ ⊢ A ≈ A[Id] : Sort@s3 }} by (symmetry; mauto 2). *)
-  (*     gen_presup H13. *)
-  (*     assert ({{ Γ ⊢ A[Id] : Sort@s3 }} -> {{ Γ ⊢ A[Id] ≈ A' : Sort@s3 }}) by (eapply H10; mauto 4). *)
-  (*     assert {{ Γ ⊢ A[Id] ≈ A' : Sort@s3 }} by mauto 2. *)
-  (*     assert {{ Γ ⊢ A ≈ A' : Sort@s3 }} by (etransitivity; mauto 2). *)
-  (*     etransitivity; mauto 2. *)
-  (*   + intros. *)
-  (*     assert {{ Δ ⊢ A[σ] ≈ A'[σ] }} by mauto 3. *)
-  (*     assert {{ Δ ⊢ A[σ] ≈ A'0 }} by (etransitivity; mauto 2). *)
-  (*     split; intros. *)
-  (*     * assert {{ Δ ⊢ A[σ] ≈ A'[σ] : K }} by (eapply H10; mauto 3). *)
-  (*       gen_presup H18. *)
-  (*       assert ({{ Δ ⊢ A[σ] : K }} -> {{ Δ ⊢ A[σ] ≈ A'0 : K }}) by (eapply H10; mauto 3). *)
-  (*       assert {{ Δ ⊢ A[σ] ≈ A'0 : K }} by mauto 2. *)
-  (*       etransitivity; mauto 3. *)
-  (*     * assert {{ Δ ⊢ A[σ] ≈ A'0 : K }} by (eapply H10; mauto 3). *)
-  (*       gen_presup H18. *)
-  (*       assert ({{ Δ ⊢ A[σ] : K }} -> {{ Δ ⊢ A[σ] ≈ A'[σ] : K }}) by (eapply H10; mauto 3). *)
-  (*       assert {{ Δ ⊢ A[σ] ≈ A'[σ] : K }} by mauto 2. *)
-  (*       etransitivity; mauto 3. *)
-        
-  (* - repeat split. *)
-  (*   + assert {{ Γ ⊢ A[Id] : Sort@s }} by mauto 3. *)
-  (*     assert ({{ Γ ⊢ A[Id] : Sort@s }} -> {{ Γ ⊢ A[Id] ≈ A' : Sort@s }}) by (eapply H4; mauto 3). *)
-  (*     assert {{ Γ ⊢ A[Id] ≈ A' : Sort@s }} by mauto 2. *)
-  (*     assert {{ Γ ⊢ A ≈ A[Id] : Sort@s }} by (symmetry; mauto 2). *)
-  (*     assert {{ Γ ⊢ A ≈ A' : Sort@s }} by (etransitivity; mauto 2). *)
-  (*     gen_presup H8; eassumption. *)
-  (*   + intros. *)
-  (*     assert {{ Δ ⊢ A[σ] ≈ A'[σ] }} by mauto 3. *)
-  (*     assert {{ Δ ⊢ A[σ] ≈ A'0 }} by (etransitivity; mauto 2). *)
-  (*     assert {{ Δ ⊢ A[σ] ≈ A'[σ] : K }} by (eapply H4; mauto 3). *)
-  (*     gen_presup H11. *)
-  (*     assert ({{ Δ ⊢ A[σ] : K }} -> {{ Δ ⊢ A[σ] ≈ A'0 : K }}) by (eapply H4; mauto 3). *)
-  (*     assert {{ Δ ⊢ A[σ] ≈ A'0 : K }} by mauto 2. *)
-  (*     etransitivity; mauto 3. *)
-  (*   + intros. *)
-  (*     assert {{ Δ ⊢ A'[σ] ≈ A[σ] }} by (symmetry; mauto 3). *)
-  (*     assert {{ Δ ⊢ A[σ] ≈ A'0 }} by (etransitivity; mauto 2). *)
-  (*     assert {{ Δ ⊢ A[σ] ≈ A'0 : K}} by (eapply H4; mauto 3). *)
-  (*     gen_presup H11. *)
-  (*     assert ({{ Δ ⊢ A[σ] : K }} -> {{ Δ ⊢ A[σ] ≈ A'[σ] : K }}) by (eapply H4; mauto 3). *)
-  (*     assert {{ Δ ⊢ A[σ] ≈ A'[σ] : K }} by mauto 2. *)
-  (*     etransitivity; mauto 3.       *)
-  (*   + intros. *)
-  (*     assert {{ Δ ⊢ A'[σ] ≈ A[σ] }} by (symmetry; mauto 3). *)
-  (*     assert {{ Δ ⊢ A[σ] ≈ A'0 }} by (eapply H5; mauto 2). *)
-  (*     etransitivity; mauto 2. *)
 Qed.
 
 Add Parametric Morphism {P} (pred_P : PredicativeSig P) s typ_rel exp_rel a (H : glu_sort_elem pred_P s typ_rel exp_rel a) Γ : (typ_rel Γ)
-    with signature wf_typ_eq Γ  ==> iff as glu_sort_elem_typ_morphism_iff1.
+    with signature wf_exp_eq Γ {{{ Sort@s }}}  ==> iff as glu_sort_elem_typ_morphism_iff1.
 Proof.
-  split; intros; eapply glu_sort_elem_typ_resp_typ_eq; mauto 2.
+  split; intros; eapply glu_sort_elem_typ_resp_exp_eq; mauto 2.
 Qed.
 
 
-Corollary glu_sort_elem_typ_resp_typ_exp_eq {P} (pred_P : PredicativeSig P) : forall s typ_rel exp_rel a,
-    {{ DG a ∈ glu_sort_elem pred_P s ↘ typ_rel ↘ exp_rel }} ->
-    forall Γ A A',
-      {{ Γ ⊢ A ® typ_rel }} ->
-      {{ Γ ⊢ A ≈ A' : Sort@s }} ->
-      {{ Γ ⊢ A' ® typ_rel }}.
-Proof.
-  intros.
-  assert {{ Γ ⊢ A ≈ A' }} by mauto 2.
-  eapply glu_sort_elem_typ_resp_typ_eq; mauto 2.
-Qed.
+(* Corollary glu_sort_elem_typ_resp_typ_exp_eq {P} (pred_P : PredicativeSig P) : forall s typ_rel exp_rel a, *)
+(*     {{ DG a ∈ glu_sort_elem pred_P s ↘ typ_rel ↘ exp_rel }} -> *)
+(*     forall Γ A A', *)
+(*       {{ Γ ⊢ A ® typ_rel }} -> *)
+(*       {{ Γ ⊢ A ≈ A' : Sort@s }} -> *)
+(*       {{ Γ ⊢ A' ® typ_rel }}. *)
+(* Proof. *)
+(*   intros. *)
+(*   assert {{ Γ ⊢ A ≈ A' }} by mauto 2. *)
+(*   eapply glu_sort_elem_typ_resp_typ_eq; mauto 2. *)
+(* Qed. *)
 
 
-Add Parametric Morphism {P} (pred_P : PredicativeSig P) s typ_rel exp_rel a (H : glu_sort_elem pred_P s typ_rel exp_rel a) Γ : (typ_rel Γ)
-    with signature wf_exp_eq Γ {{{ Sort@s }}} ==> iff as glu_sort_elem_typ_morphism_iff1'.
-Proof.
-  split; intros; eapply glu_sort_elem_typ_resp_typ_exp_eq; mauto 2.
-Qed.
+(* Add Parametric Morphism {P} (pred_P : PredicativeSig P) s typ_rel exp_rel a (H : glu_sort_elem pred_P s typ_rel exp_rel a) Γ : (typ_rel Γ) *)
+(*     with signature wf_exp_eq Γ {{{ Sort@s }}} ==> iff as glu_sort_elem_typ_morphism_iff1'. *)
+(* Proof. *)
+(*   split; intros; eapply glu_sort_elem_typ_resp_typ_exp_eq; mauto 2. *)
+(* Qed. *)
 
 
-Lemma glu_sort_elem_trm_resp_typ_eq {P} (pred_P : PredicativeSig P) : forall s typ_rel exp_rel a,
+Lemma glu_sort_elem_trm_resp_typ_exp_eq {P} (pred_P : PredicativeSig P) : forall s typ_rel exp_rel a,
     {{ DG a ∈ glu_sort_elem pred_P s ↘ typ_rel ↘ exp_rel }} ->
     forall Γ M A m A',
       {{ Γ ⊢ M : A ® m ∈ exp_rel }} ->
-      {{ Γ ⊢ A ≈ A' }} ->
+      {{ Γ ⊢ A ≈ A' : Sort@s }} ->
       {{ Γ ⊢ M : A' ® m ∈ exp_rel }}.
 Proof.
   simpl.
   induction 1 using glu_sort_elem_ind; intros;
     simpl_glu_rel; repeat split; intros; mauto 3.
   
-  (* - assert {{ Δ ⊢ A[σ] ≈ A'[σ] }} by mauto 3. *)
-  (*   assert {{ Δ ⊢ A[σ] ≈ A'0 }} by (etransitivity; mauto 2). *)
-  (*   assert {{ Δ ⊢ A[σ] ≈ A'[σ] : K }} by (eapply H5; mauto 3). *)
-  (*   gen_presup H13. *)
-  (*   assert ({{ Δ ⊢ A[σ] : K }} -> {{ Δ ⊢ A[σ] ≈ A'0 : K }}) by (eapply H5; mauto 3). *)
-  (*   assert {{ Δ ⊢ A[σ] ≈ A'0 : K }} by mauto 2. *)
-  (*   etransitivity; mauto 3. *)
-  (* - assert {{ Δ ⊢ A[σ] ≈ A'[σ] }} by mauto 3. *)
-  (*   assert {{ Δ ⊢ A[σ] ≈ A'0 }} by (etransitivity; mauto 2). *)
-  (*   assert {{ Δ ⊢ A[σ] ≈ A'0 : K }} by (eapply H5; mauto 2). *)
-  (*   gen_presup H13. *)
-  (*   assert ({{ Δ ⊢ A[σ] : K }} -> {{ Δ ⊢ A[σ] ≈ A'[σ] : K }}) by (eapply H5; mauto 3). *)
-  (*   assert {{ Δ ⊢ A[σ] ≈ A'[σ] : K }} by mauto 2. *)
-  (*   etransitivity; mauto 3. *)
-  (* (* - assert ({{ Δ ⊢ M[σ] : B }} -> {{ Δ ⊢ M[σ] ≈ M' : B}}) by (eapply H6; mauto 3). *) *)
-  (* (*   mauto 2. *) *)
-  (* (* - eapply H6; mauto 3. *) *)
   - firstorder.
-
   - econstructor; mauto 3.
-    (* + assert {{ Γ ⊢ A ≈ A[Id] : Sort@s3 }} by (symmetry; mauto 2). *)
-    (*   gen_presup H15. *)
-    (*   assert ({{ Γ ⊢ A[Id] : Sort@s3 }} -> {{ Γ ⊢ A[Id] ≈ A' : Sort@s3 }}) by (eapply H12; mauto 3). *)
-    (*   assert {{ Γ ⊢ A[Id] ≈ A' : Sort@s3 }} by mauto 2. *)
-    (*   assert {{ Γ ⊢ A ≈ A' : Sort@s3 }} by (etransitivity; mauto 2). *)
-    (*   etransitivity; mauto 2. *)
-    (* + intros. *)
-    (*   assert {{ Δ ⊢ A[σ] ≈ A'[σ] }} by mauto 3. *)
-    (*   assert {{ Δ ⊢ A[σ] ≈ A'0 }} by (etransitivity; mauto 2). *)
-    (*   split; intros. *)
-    (*   * assert {{ Δ ⊢ A'[σ] ≈ A[σ] : K }} by (symmetry; eapply H12; mauto 2). *)
-    (*     gen_presup H20. *)
-    (*     assert ({{ Δ ⊢ A[σ] : K }} -> {{ Δ ⊢ A[σ] ≈ A'0 : K }}) by (eapply H12; mauto 2). *)
-    (*     assert {{ Δ ⊢ A[σ] ≈ A'0 : K }} by mauto 2. *)
-    (*     etransitivity; mauto 2. *)
-    (*   * assert {{ Δ ⊢ A'0 ≈ A[σ] : K }} by (symmetry; eapply H12; mauto 2). *)
-    (*     gen_presup H20. *)
-    (*     assert ({{ Δ ⊢ A[σ] : K }} -> {{ Δ ⊢ A[σ] ≈ A'[σ] : K }}) by (eapply H12; mauto 2). *)
-    (*     assert {{ Δ ⊢ A[σ] ≈ A'[σ] : K }} by mauto 2. *)
-    (*     etransitivity; mauto 2. *)
-      
-  (* - assert ({{ Γ ⊢ A[Id] : Sort@s }} -> {{ Γ ⊢ A[Id] ≈ A' : Sort@s }}) by (eapply H4; mauto 3). *)
-  (*   assert {{ Γ ⊢ A[Id] : Sort@s }} by mauto 3. *)
-  (*   assert {{ Γ ⊢ A[Id] ≈ A' : Sort@s }} by mauto 3. *)
-  (*   gen_presup H11; eassumption. *)
-  (* - assert {{ Δ ⊢ A[σ] ≈ A'[σ] }} by mauto 3. *)
-  (*   assert {{ Δ ⊢ A[σ] ≈ A'0 }} by (etransitivity; mauto 2). *)
-  (*   assert {{ Δ ⊢ A'[σ] ≈ A[σ] : K }} by (symmetry; eapply H4; mauto 2). *)
-  (*   gen_presup H14. *)
-  (*   assert ({{ Δ ⊢ A[σ] : K }} -> {{ Δ ⊢ A[σ] ≈ A'0 : K }}) by (eapply H4; mauto 2). *)
-  (*   assert {{ Δ ⊢ A[σ] ≈ A'0 : K }} by mauto 2. *)
-  (*   etransitivity; mauto 2. *)
-  (* - assert {{ Δ ⊢ A[σ] ≈ A'[σ] }} by mauto 3. *)
-  (*   assert {{ Δ ⊢ A[σ] ≈ A'0 }} by (etransitivity; mauto 2). *)
-  (*   assert {{ Δ ⊢ A'0 ≈ A[σ] : K }} by (symmetry; eapply H4; mauto 2). *)
-  (*   gen_presup H14. *)
-  (*   assert ({{ Δ ⊢ A[σ] : K }} -> {{ Δ ⊢ A[σ] ≈ A'[σ] : K }}) by (eapply H4; mauto 2). *)
-  (*   assert {{ Δ ⊢ A[σ] ≈ A'[σ] : K }} by mauto 2. *)
-  (*   etransitivity; mauto 2. *)
-    
   - transitivity {{{ A[σ] }}}; mauto 4.
-    (* assert {{ Δ ⊢ A'[σ] ≈ A[σ] }} by (symmetry; mauto 3). *)
-    (* assert {{ Δ ⊢ A[σ] ≈ A'0 }} by (eapply H8; mauto 2). *)
-    (* etransitivity; mauto 2. *)
   - assert {{ Δ ⊢ M[σ] ≈ M' : A[σ] }} by mauto 2.
-    eapply wf_exp_eq_conv'; mauto 3.
+    eapply wf_exp_eq_conv'; mauto 4.
 Qed.
 
 Add Parametric Morphism {P} (pred_P : PredicativeSig P) s typ_rel exp_rel a (H : glu_sort_elem pred_P s typ_rel exp_rel a) Γ : (exp_rel Γ)
-    with signature wf_typ_eq Γ  ==> eq ==> eq ==> iff as glu_sort_elem_trm_morphism_iff1.
-Proof.
-  split; intros;
-    eapply glu_sort_elem_trm_resp_typ_eq;
-    mauto 2.
-Qed.
-
-
-Corollary glu_sort_elem_trm_resp_typ_exp_eq {P} (pred_P : PredicativeSig P) : forall s typ_rel exp_rel a,
-    {{ DG a ∈ glu_sort_elem pred_P s ↘ typ_rel ↘ exp_rel }} ->
-    forall Γ M A m A',
-      {{ Γ ⊢ M : A ® m ∈ exp_rel }} ->
-      {{ Γ ⊢ A ≈ A' : Sort@s }} ->
-      {{ Γ ⊢ M : A' ® m ∈ exp_rel }}.
-Proof.
-  intros.
-  eapply glu_sort_elem_trm_resp_typ_eq; mauto 2.
-Qed.
-
-Add Parametric Morphism {P} (pred_P : PredicativeSig P) s typ_rel exp_rel a (H : glu_sort_elem pred_P s typ_rel exp_rel a) Γ : (exp_rel Γ)
-    with signature wf_exp_eq Γ {{{ Sort@s }}} ==> eq ==> eq ==> iff as glu_sort_elem_trm_morphism_iff1'.
+    with signature wf_exp_eq Γ {{{ Sort@s }}}  ==> eq ==> eq ==> iff as glu_sort_elem_trm_morphism_iff1.
 Proof.
   split; intros;
     eapply glu_sort_elem_trm_resp_typ_exp_eq;
     mauto 2.
 Qed.
+
+
+(* Corollary glu_sort_elem_trm_resp_typ_exp_eq {P} (pred_P : PredicativeSig P) : forall s typ_rel exp_rel a, *)
+(*     {{ DG a ∈ glu_sort_elem pred_P s ↘ typ_rel ↘ exp_rel }} -> *)
+(*     forall Γ M A m A', *)
+(*       {{ Γ ⊢ M : A ® m ∈ exp_rel }} -> *)
+(*       {{ Γ ⊢ A ≈ A' : Sort@s }} -> *)
+(*       {{ Γ ⊢ M : A' ® m ∈ exp_rel }}. *)
+(* Proof. *)
+(*   intros. *)
+(*   eapply glu_sort_elem_trm_resp_typ_eq; mauto 2. *)
+(* Qed. *)
+
+(* Add Parametric Morphism {P} (pred_P : PredicativeSig P) s typ_rel exp_rel a (H : glu_sort_elem pred_P s typ_rel exp_rel a) Γ : (exp_rel Γ) *)
+(*     with signature wf_exp_eq Γ {{{ Sort@s }}} ==> eq ==> eq ==> iff as glu_sort_elem_trm_morphism_iff1'. *)
+(* Proof. *)
+(*   split; intros; *)
+(*     eapply glu_sort_elem_trm_resp_typ_exp_eq; *)
+(*     mauto 2. *)
+(* Qed. *)
 
 
 Lemma glu_sort_elem_typ_resp_ctx_eq {P} (pred_P : PredicativeSig P) : forall s typ_rel exp_rel a,
@@ -278,9 +238,6 @@ Proof.
   induction 1 using glu_sort_elem_ind; intros;
     simpl_glu_rel; mauto 2;
     econstructor; mauto 4.
-  (* - assert {{ ⊢ Γ, IT ≈ Δ, IT }} by mauto 4. *)
-  (*   mauto 2. *)
-  (* - split; intros; mauto 4. *)
 Qed.
 
 Add Parametric Morphism {P} (pred_P : PredicativeSig P) s typ_rel exp_rel a (H : glu_sort_elem pred_P s typ_rel exp_rel a) : typ_rel
@@ -300,8 +257,6 @@ Proof.
   intros.
   inversion_clear H.
   econstructor; mauto 4.
-  (* assert {{ ⊢ Γ, IT ≈ Δ, IT }} by mauto 4. *)
-  (* mauto 2. *)
 Qed.
 
 
@@ -316,26 +271,14 @@ Proof.
   induction 1 using glu_sort_elem_ind; intros;
     simpl_glu_rel; mauto 2.
   - repeat split; mauto 3.
-    (* + assert {{ Δ0 ⊢w σ : Γ }} by mauto 3. *)
-    (*   eapply H5; mauto 3. *)
-    (* + assert {{ Δ0 ⊢w σ : Γ }} by mauto 3. *)
-    (*   eapply H5; mauto 3. *)
-    (* (* + eapply H6; mauto 3. *) *)
-    (* (* + eapply H6; mauto 3. *) *)
-    + do 2 eexists; split; mauto 4.    
-      eapply glu_sort_elem_typ_resp_ctx_eq; mauto 2.
+    do 2 eexists; split; mauto 4.    
+    eapply glu_sort_elem_typ_resp_ctx_eq; mauto 2.
 
   - eapply glu_sort_elem_trm_resp_ctx_eq_pi_helper; mauto.
   - econstructor; mauto 4.
     repeat split; mauto 2; intros.
-    (* + intros. *)
-    (*   assert {{ Δ0 ⊢w σ : Γ }} by mauto 3. *)
-    (*   assert ({{ Δ0 ⊢ A[σ] : K }} -> {{ Δ0 ⊢ A[σ] ≈ A' : K }}) by (eapply H4; mauto 3). *)
-    (*   mauto 2. *)
-    (* + intros. *)
-    (*   assert {{ Δ0 ⊢w σ : Γ }} by mauto 3. *)
-    (*   eapply H4; mauto 3. *)
-    + mauto 4.
+    mauto 4.
+  - split; mauto 3.
 Qed.
 
 Add Parametric Morphism {P} (pred_P : PredicativeSig P) s typ_rel exp_rel a (H : glu_sort_elem pred_P s typ_rel exp_rel a) : exp_rel
@@ -356,6 +299,8 @@ Proof.
   simpl.
   induction 1 using glu_sort_elem_ind; intros;
     simpl_glu_rel; mauto 4.
+  enough {{ Γ ⊢ M : ℕ }} by mauto 4.
+  mauto 2.
 Qed.
 
 Lemma glu_sort_elem_per_sort {P} (pred_P : PredicativeSig P) : forall s typ_rel exp_rel a,
@@ -363,12 +308,9 @@ Lemma glu_sort_elem_per_sort {P} (pred_P : PredicativeSig P) : forall s typ_rel 
     {{ Dom a ≈ a ∈ per_sort pred_P s }}.
 Proof.
   simpl.
-  induction 1 using glu_sort_elem_ind; intros; eexists.
-  - eapply per_sort_elem_core_sort'; mauto 2.
-    reflexivity.
-  - try solve [per_sort_elem_econstructor; mauto 3; try reflexivity].
-    eassumption.
-  - try solve [per_sort_elem_econstructor; mauto 3; try reflexivity].  
+  induction 1 using glu_sort_elem_ind; intros; eexists;
+    only 1: (eapply per_sort_elem_core_sort'; mauto 2; reflexivity);
+    try solve [per_sort_elem_econstructor; mauto 3; try reflexivity]; eassumption.
 Qed.
 
 #[export]
@@ -383,7 +325,7 @@ Lemma glu_sort_elem_per_elem {P} (pred_P : PredicativeSig P) : forall s typ_rel 
 Proof.
   simpl.
   induction 1 using glu_sort_elem_ind; intros.
-  2,3: match_by_head (@per_sort_elem P) ltac:(fun H => directed invert_per_sort_elem H);
+  2-4: match_by_head (@per_sort_elem P) ltac:(fun H => directed invert_per_sort_elem H);
     simpl_glu_rel;
     try fold (per_sort pred_P s' m m);
     mauto 4.
@@ -450,7 +392,7 @@ Lemma glu_sort_elem_trm_sort_lvl {P} (pred_P : PredicativeSig P) : forall s typ_
     {{ DG a ∈ glu_sort_elem pred_P s ↘ typ_rel ↘ exp_rel }} ->
     forall Γ M A m,
       {{ Γ ⊢ M : A ® m ∈ exp_rel }} ->
-      {{ Γ ⊢ A }}.
+      {{ Γ ⊢ A : Sort@s }}.
 Proof.
   intros. eapply glu_sort_elem_sort_lvl; [| eapply glu_sort_elem_trm_typ]; eassumption.
 Qed.
@@ -467,31 +409,10 @@ Proof.
     simpl_glu_rel;
     repeat split; mauto 3.
 
-  (* - eapply H5; mauto 3. *)
-  (* - eapply H5; mauto 3. *)
-  (* - intros. *)
-  (*   assert {{ Γ ⊢ M ≈ M' }} by mauto 4. *)
-  (*   assert {{ Δ ⊢ M[σ] ≈ M'[σ] }} by mauto 3. *)
-  (*   assert {{ Δ ⊢ M[σ] ≈ M'[σ] : B }} by (eapply H6; mauto 3). *)
-  (*   gen_presup H13. *)
-  (*   assert {{ Δ ⊢ M[σ] ≈ M'0 }} by (transitivity {{{ M'[σ] }}}; mauto 3). *)
-  (*   assert ({{ Δ ⊢ M[σ] : B }} -> {{ Δ ⊢ M[σ] ≈ M'0 : B }}) by (eapply H6; mauto 3). *)
-  (*   assert {{ Δ ⊢ M[σ] ≈ M'0 : B }} by mauto 2. *)
-  (*   transitivity {{{ M[σ] }}}; mauto 2. *)
-  (* - intros. *)
-  (*   assert {{ Γ ⊢ M ≈ M' }} by mauto 4. *)
-  (*   assert {{ Δ ⊢ M[σ] ≈ M'[σ] }} by mauto 3. *)
-  (*   assert {{ Δ ⊢ M[σ] ≈ M'0 }} by (transitivity {{{ M'[σ] }}}; mauto 3). *)
-  (*   assert {{ Δ ⊢ M[σ] ≈ M'0 : B }} by (eapply H6; mauto 3). *)
-  (*   gen_presup H14.     *)
-  (*   assert ({{ Δ ⊢ M[σ] : B }} -> {{ Δ ⊢ M[σ] ≈ M'[σ] : B }}) by (eapply H6; mauto 3). *)
-  (*   assert {{ Δ ⊢ M[σ] ≈ M'[σ] : B }} by mauto 2. *)
-  (*   transitivity {{{ M[σ] }}}; mauto 2. *)
   - repeat eexists; try split; eauto.
-    eapply glu_sort_elem_typ_resp_typ_eq; mauto.
+    eapply glu_sort_elem_typ_resp_exp_eq; mauto.
 
   - econstructor; eauto.
-    assert ({{ Γ ⊢ IT : Sort@s1 }} /\ {{ Γ, IT ⊢ OT : Sort@s2 }}) by (gen_presup H9; mauto 2).
     destruct_conjs.
     match_by_head (@per_sort_elem P) ltac:(fun H => directed invert_per_sort_elem H).
     intros.
@@ -505,23 +426,14 @@ Proof.
     assert {{ Δ, IT[σ] ⊢ OT[q σ] : Sort@s2 }} by mauto 4.
     eapply wf_exp_eq_sub_cong with (Γ := Δ) in Hty; [| eapply sub_eq_refl; mauto 3].
     autorewrite with mcpts in Hty.
-    eapply wf_exp_eq_app_cong with (N := N) (N' := N) in Hty; mauto 2.  (* try pi_sort_level_tac; [|mauto 2]. *)
-    (* autorewrite with mcpts in Hty. *)
+    eapply wf_exp_eq_app_cong with (N := N) (N' := N) in Hty; mauto 2.
     assert ({{ Δ ⊢ OT[q σ][Id,,N] ≈ OT[σ,,N] }}) by mauto 4.
     mauto.
-    (* + eassumption. *)
-    (* + assert {{ Δ, IT[σ] ⊢s q σ : Γ, IT }} by mauto 4. *)
-    (*   eapply wf_conv with (A := {{{ Sort@s2[q σ] }}}); mauto 4. *)
-    (* + mauto. *)
-
-  (* - intros. *)
-  (*   assert ({{ Δ ⊢ A[σ] : K }} -> {{ Δ ⊢ A[σ] ≈ A' : K }}) by (eapply H4; mauto 3). *)
-  (*   mauto 2.     *)
-  (* - intros. *)
-  (*   eapply H4; mauto 3. *)
 
   - intros.
     enough {{ Δ ⊢ M[σ] ≈ M'[σ] : A[σ] }}; mauto 4.
+
+  - mauto 4.
 Qed.
 
 Add Parametric Morphism {P} (pred_P : PredicativeSig P) s typ_rel exp_rel a (H : glu_sort_elem pred_P s typ_rel exp_rel a) Γ T : (exp_rel Γ T)
@@ -535,8 +447,8 @@ Qed.
 
 Lemma glu_sort_elem_core_sort' {P} (pred_P : PredicativeSig P) : forall s' s typ_rel el_rel,
     Ax P s' s ->
-    (typ_rel <∙> sort_glu_typ_pred pred_P s') ->
-    (el_rel <∙> sort_glu_exp_pred pred_P s') ->
+    (typ_rel <∙> sort_glu_typ_pred pred_P s' s) ->
+    (el_rel <∙> sort_glu_exp_pred pred_P s' s) ->
     {{ DG Sort@s' ∈ glu_sort_elem pred_P s ↘ typ_rel ↘ el_rel }}.
 Proof.
   intros.
@@ -551,7 +463,7 @@ Ltac glu_sort_elem_econstructor :=
 
 Lemma glu_sort_elem_sort_simple_constructor {P} (pred_P : PredicativeSig P) : forall {s' s},
     Ax P s' s ->
-    glu_sort_elem pred_P s (sort_glu_typ_pred pred_P s') (sort_glu_exp_pred pred_P s') d{{{ Sort@s' }}}.
+    glu_sort_elem pred_P s (sort_glu_typ_pred pred_P s' s) (sort_glu_exp_pred pred_P s' s) d{{{ Sort@s' }}}.
 Proof.
   intros.
   glu_sort_elem_econstructor; mauto; reflexivity.
@@ -603,7 +515,7 @@ Proof with mautosolve.
 Qed.
 
 (** *** Morphism instances for [neut_glu_*_pred]s *)
-Add Parametric Morphism {P : PtsSig} : (@neut_glu_typ_pred P)
+Add Parametric Morphism {P : PtsSig} (s : P) : (neut_glu_typ_pred s)
     with signature per_bot ==> eq ==> eq ==> iff as neut_glu_typ_pred_morphism_iff.
 Proof with mautosolve.
   split; intros []; econstructor; intuition;
@@ -611,13 +523,13 @@ Proof with mautosolve.
     functional_read_rewrite_clear; intuition.
 Qed.
 
-Add Parametric Morphism {P : PtsSig} : (@neut_glu_typ_pred P)
+Add Parametric Morphism {P : PtsSig} (s : P) : (neut_glu_typ_pred s)
     with signature per_bot ==> glu_typ_pred_equivalence P as neut_glu_typ_pred_morphism_glu_typ_pred_equivalence.
 Proof with mautosolve.
   split; apply neut_glu_typ_pred_morphism_iff; mauto.
 Qed.
 
-Add Parametric Morphism {P : PtsSig} : (@neut_glu_exp_pred P)
+Add Parametric Morphism {P : PtsSig} (s : P) : (neut_glu_exp_pred s)
     with signature per_bot ==> eq ==> eq ==> eq ==> eq ==> iff as neut_glu_exp_pred_morphism_iff.
 Proof with mautosolve.
   split; intros []; econstructor; intuition;
@@ -626,7 +538,7 @@ Proof with mautosolve.
     match_by_head (@per_bot P) ltac:(fun H => rewrite H in *); eassumption.
 Qed.
 
-Add Parametric Morphism {P : PtsSig} : (@neut_glu_exp_pred P)
+Add Parametric Morphism {P : PtsSig} (s : P) : (neut_glu_exp_pred s)
     with signature per_bot ==> glu_exp_pred_equivalence P as neut_glu_exp_pred_morphism_glu_exp_pred_equivalence.
 Proof with mautosolve.
   split; apply neut_glu_exp_pred_morphism_iff; mauto.
@@ -658,7 +570,7 @@ Proof with mautosolve.
 Qed.
 
 
-Lemma functional_glu_sort_elem_helper {P} (pred_P : PredicativeSig P) : forall s a typ_rel typ_rel' exp_rel exp_rel',
+Lemma functional_glu_sort_elem {P} (pred_P : PredicativeSig P) : forall s a typ_rel typ_rel' exp_rel exp_rel',
     {{ DG a ∈ glu_sort_elem pred_P s ↘ typ_rel ↘ exp_rel }} ->
     {{ DG a ∈ glu_sort_elem pred_P s ↘ typ_rel' ↘ exp_rel' }} ->
     (typ_rel <∙> typ_rel') /\ (exp_rel <∙> exp_rel').
@@ -668,88 +580,90 @@ Proof.
   induction Ha using glu_sort_elem_ind; intros; basic_invert_glu_sort_elem Ha';
     apply_predicate_equivalence; try solve [split; reflexivity].
 
-  (* destruct_conjs. *)
-  assert ((IP <∙> IP0) /\ (IEL <∙> IEL0)) as [].
-  { 
-    assert ((pred_rel pred_P s1 s3 \/ s1 = s3) /\ (pred_rel pred_P s2 s3 \/ s2 = s3)) by (eapply ord_ru; mauto).
-    destruct_conjs.
-    destruct H4.
-    - assert (glu_sort_elem pred_P s1 IP0 IEL0 a) by mauto.
-      apply (IHHa IEL0 IP0 H11).
-    - assert (glu_sort_elem pred_P s1 IP0 IEL0 a) by (subst; mauto).
-      apply (IHHa IEL0 IP0 H11).
-  }
-  apply_predicate_equivalence.
-  handle_per_sort_elem_irrel.
-  (on_all_hyp: fun H => directed invert_per_sort_elem H).
-  handle_per_sort_elem_irrel.
-  split; [intros Γ C | intros Γ M C m].
-  - split; intros []; econstructor; intuition;
-      [rename equiv_m into equiv0_m; assert (equiv_m : in_rel m m) by intuition
-      | assert (equiv0_m : in_rel0 m m) by intuition ];
-      destruct_rel_mod_eval;
-      functional_eval_rewrite_clear;
-      assert ((OP m equiv_m <∙> OP0 m equiv0_m) /\ (OEL m equiv_m <∙> OEL0 m equiv0_m)) as [] by
-        (assert ((pred_rel pred_P s1 s3 \/ s1 = s3) /\ (pred_rel pred_P s2 s3 \/ s2 = s3)) by (eapply ord_ru; mauto);
-         assert ((s2 = s3 -> glu_sort_elem pred_P s3 (OP0 m equiv0_m) (OEL0 m equiv0_m) a0) /\
-                   (pred_rel pred_P s2 s3 -> glu_sort_elem pred_P s2 (OP0 m equiv0_m) (OEL0 m equiv0_m) a0)) by mauto;
-         destruct_conjs;
-         destruct H20;
-         [
-           assert (glu_sort_elem pred_P s2 (OP0 m equiv0_m) (OEL0 m equiv0_m) a0) by mauto;
-           eapply H2; mauto
-         |
-           assert (glu_sort_elem pred_P s2 (OP0 m equiv0_m) (OEL0 m equiv0_m) a0) by (subst; mauto);
-           eapply H2; mauto
-        ]);
-      intuition.
+  - assert ((IP <∙> IP0) /\ (IEL <∙> IEL0)) as [].
+    { 
+      assert ((pred_rel pred_P s1 s3 \/ s1 = s3) /\ (pred_rel pred_P s2 s3 \/ s2 = s3)) by (eapply ord_ru; mauto).
+      destruct_conjs.
+      destruct H4.
+      + assert (glu_sort_elem pred_P s1 IP0 IEL0 a) by mauto.
+        apply (IHHa IEL0 IP0 H11).
+      + assert (glu_sort_elem pred_P s1 IP0 IEL0 a) by (subst; mauto).
+        apply (IHHa IEL0 IP0 H11).
+    }
+    apply_predicate_equivalence.
+    handle_per_sort_elem_irrel.
+    (on_all_hyp: fun H => directed invert_per_sort_elem H).
+    handle_per_sort_elem_irrel.
+    split; [intros Γ C | intros Γ M C m].
+    + split; intros []; econstructor; intuition;
+        [rename equiv_m into equiv0_m; assert (equiv_m : in_rel m m) by intuition
+        | assert (equiv0_m : in_rel0 m m) by intuition ];
+        destruct_rel_mod_eval;
+        functional_eval_rewrite_clear;
+        assert ((OP m equiv_m <∙> OP0 m equiv0_m) /\ (OEL m equiv_m <∙> OEL0 m equiv0_m)) as [] by
+          (assert ((pred_rel pred_P s1 s3 \/ s1 = s3) /\ (pred_rel pred_P s2 s3 \/ s2 = s3)) by (eapply ord_ru; mauto);
+           assert ((s2 = s3 -> glu_sort_elem pred_P s3 (OP0 m equiv0_m) (OEL0 m equiv0_m) a0) /\
+                     (pred_rel pred_P s2 s3 -> glu_sort_elem pred_P s2 (OP0 m equiv0_m) (OEL0 m equiv0_m) a0)) by mauto;
+           destruct_conjs;
+           destruct H20;
+           [
+             assert (glu_sort_elem pred_P s2 (OP0 m equiv0_m) (OEL0 m equiv0_m) a0) by mauto;
+             eapply H2; mauto
+           |
+             assert (glu_sort_elem pred_P s2 (OP0 m equiv0_m) (OEL0 m equiv0_m) a0) by (subst; mauto);
+             eapply H2; mauto
+          ]);
+        intuition.
     
-  - split; intros []; econstructor; intuition;
+    + split; intros []; econstructor; intuition;
         [rename equiv_n into equiv0_n; assert (equiv_n : in_rel n n) by intuition
         | assert (equiv0_n : in_rel0 n n) by intuition];
         destruct_rel_mod_eval;
         [assert (exists m0n, {{ $| m0 & n |↘ m0n }} /\ {{ Δ ⊢ M0[σ] N : OT[σ,,N] ® m0n ∈ OEL n equiv_n }}) by intuition
         | assert (exists m0n, {{ $| m0 & n |↘ m0n }} /\ {{ Δ ⊢ M0[σ] N : OT[σ,,N] ® m0n ∈ OEL0 n equiv0_n }}) by intuition];
         destruct_conjs;
-      assert ((OP n equiv_n <∙> OP0 n equiv0_n) /\ (OEL n equiv_n <∙> OEL0 n equiv0_n)) as [] by
-        (
-          functional_eval_rewrite_clear;
-          assert ((pred_rel pred_P s1 s3 \/ s1 = s3) /\ (pred_rel pred_P s2 s3 \/ s2 = s3)) by (eapply ord_ru; mauto);
-          assert ((s2 = s3 -> glu_sort_elem pred_P s3 (OP0 n equiv0_n) (OEL0 n equiv0_n) a0) /\
-                    (pred_rel pred_P s2 s3 -> glu_sort_elem pred_P s2 (OP0 n equiv0_n) (OEL0 n equiv0_n) a0)) by mauto;
-          destruct_conjs;
-          destruct H25;
-          [
-            assert (glu_sort_elem pred_P s2 (OP0 n equiv0_n) (OEL0 n equiv0_n) a0) by mauto;
-            eapply H2; mauto
-          |
-            assert (glu_sort_elem pred_P s2 (OP0 n equiv0_n) (OEL0 n equiv0_n) a0) by (subst; mauto);
-            eapply H2; mauto
+        assert ((OP n equiv_n <∙> OP0 n equiv0_n) /\ (OEL n equiv_n <∙> OEL0 n equiv0_n)) as [] by
+          (
+            functional_eval_rewrite_clear;
+            assert ((pred_rel pred_P s1 s3 \/ s1 = s3) /\ (pred_rel pred_P s2 s3 \/ s2 = s3)) by (eapply ord_ru; mauto);
+            assert ((s2 = s3 -> glu_sort_elem pred_P s3 (OP0 n equiv0_n) (OEL0 n equiv0_n) a0) /\
+                      (pred_rel pred_P s2 s3 -> glu_sort_elem pred_P s2 (OP0 n equiv0_n) (OEL0 n equiv0_n) a0)) by mauto;
+            destruct_conjs;
+            destruct H25;
+            [
+              assert (glu_sort_elem pred_P s2 (OP0 n equiv0_n) (OEL0 n equiv0_n) a0) by mauto;
+              eapply H2; mauto
+            |
+              assert (glu_sort_elem pred_P s2 (OP0 n equiv0_n) (OEL0 n equiv0_n) a0) by (subst; mauto);
+              eapply H2; mauto
           ]);
-      eexists; split; intuition.
+        eexists; split; intuition.
+
+  - split; try reflexivity.
+    split; intros; inversion_clear H; econstructor; mauto 2.
 Qed.
 
-Lemma glu_sort_elem_sort_irrel {P} (pred_P : PredicativeSig P) : forall {s s' a typ_rel typ_rel'  exp_rel exp_rel'},
-    {{ DG a ∈ glu_sort_elem pred_P s ↘ typ_rel ↘ exp_rel }} ->
-    {{ DG a ∈ glu_sort_elem pred_P s' ↘ typ_rel' ↘ exp_rel' }} ->
-    {{ DG a ∈ glu_sort_elem pred_P s ↘ typ_rel' ↘ exp_rel' }}.
-Proof.  
-  intros * Hglu Hglu';
-    basic_invert_glu_sort_elem Hglu;
-    basic_invert_glu_sort_elem Hglu';
-    simpl_glu_rel;
-    glu_sort_elem_econstructor; mauto 3.
-Qed.  
+(* Lemma glu_sort_elem_sort_irrel {P} (pred_P : PredicativeSig P) : forall {s s' a typ_rel typ_rel'  exp_rel exp_rel'}, *)
+(*     {{ DG a ∈ glu_sort_elem pred_P s ↘ typ_rel ↘ exp_rel }} -> *)
+(*     {{ DG a ∈ glu_sort_elem pred_P s' ↘ typ_rel' ↘ exp_rel' }} -> *)
+(*     {{ DG a ∈ glu_sort_elem pred_P s ↘ typ_rel' ↘ exp_rel' }}. *)
+(* Proof.   *)
+(*   intros * Hglu Hglu'; *)
+(*     basic_invert_glu_sort_elem Hglu; *)
+(*     basic_invert_glu_sort_elem Hglu'; *)
+(*     simpl_glu_rel;     *)
+(*     glu_sort_elem_econstructor; mauto 3. *)
+(* Qed. *)
   
-Lemma functional_glu_sort_elem {P} (pred_P : PredicativeSig P) : forall s s' a typ_rel typ_rel' exp_rel exp_rel',
-    {{ DG a ∈ glu_sort_elem pred_P s ↘ typ_rel ↘ exp_rel }} ->
-    {{ DG a ∈ glu_sort_elem pred_P s' ↘ typ_rel' ↘ exp_rel' }} ->
-    (typ_rel <∙> typ_rel') /\ (exp_rel <∙> exp_rel').
-Proof.
-  intros.
-  assert {{ DG a ∈ glu_sort_elem pred_P s ↘ typ_rel' ↘ exp_rel' }} by (eapply glu_sort_elem_sort_irrel; mauto 2).
-  eapply functional_glu_sort_elem_helper; mauto 2.
-Qed.
+(* Lemma functional_glu_sort_elem {P} (pred_P : PredicativeSig P) : forall s s' a typ_rel typ_rel' exp_rel exp_rel', *)
+(*     {{ DG a ∈ glu_sort_elem pred_P s ↘ typ_rel ↘ exp_rel }} -> *)
+(*     {{ DG a ∈ glu_sort_elem pred_P s' ↘ typ_rel' ↘ exp_rel' }} -> *)
+(*     (typ_rel <∙> typ_rel') /\ (exp_rel <∙> exp_rel'). *)
+(* Proof. *)
+(*   intros. *)
+(*   assert {{ DG a ∈ glu_sort_elem pred_P s ↘ typ_rel' ↘ exp_rel' }} by (eapply glu_sort_elem_sort_irrel; mauto 2). *)
+(*   eapply functional_glu_sort_elem_helper; mauto 2. *)
+(* Qed. *)
 
 
 
@@ -950,6 +864,24 @@ Ltac invert_glu_sort_elem H :=
    destruct H as [? [? [? [? [? [? [? [? []]]]]]]]])
   + basic_invert_glu_sort_elem H.
 
+Lemma glu_nat_resp_per_nat {P} {s} (r : Ru_nat P s) : forall m n,
+    {{ Dom m ≈ n ∈ per_nat }} ->
+    forall Γ M,
+      glu_nat r Γ M m ->
+      glu_nat r Γ M n.
+Proof.
+  induction 1; intros; progressive_inversion; mauto 3.
+  econstructor.
+  - mauto using (PER_refl2 _ per_bot).
+  - intros.
+    specialize (H (length Δ)).
+    destruct_all.
+    functional_read_rewrite_clear.
+    mauto.
+Qed.
+
+#[local]
+Hint Resolve glu_nat_resp_per_nat : mcpts.
 
 #[local]
 Ltac resp_per_IH :=
@@ -990,10 +922,6 @@ Proof.
     mauto 3.
 
   - repeat split; eauto.
-    (* + eapply H3; mauto 3. *)
-    (* + eapply H3; mauto 3. *)
-    (* + eapply H4; mauto 3. *)
-    (* + eapply H4; mauto 3. *)
     + unfold glu_sort_typ_rec in *.
       destruct_conjs.
       do 2 eexists; split; mauto.
@@ -1038,8 +966,8 @@ Proof.
       destruct (H15 _ _ _ _ H20 H21 equiv_n) as [? []].
       destruct (H16 _ _ equiv_n) as [].
       simplify_evals.
-      eauto.
-  
+      eauto.   
+      
   - apply neut_glu_typ_pred_morphism_glu_typ_pred_equivalence.
     eassumption.
   - apply neut_glu_exp_pred_morphism_glu_exp_pred_equivalence.
@@ -1049,7 +977,7 @@ Proof.
     econstructor; unfold neut_glu_typ_pred; mauto 3.
 
     intros.
-    specialize (H1 (length Δ)).    
+    specialize (H9 (length Δ)).    
     destruct_all.
     functional_read_rewrite_clear.
     mauto.
@@ -1151,8 +1079,13 @@ Proof.
       intros.
       (on_all_hyp: destruct_rel_by_assumption in_rel).
       econstructor; mauto.
+      
   - destruct_conjs.
     saturate_refl.
+    exists (nat_glu_typ_pred r); exists (nat_glu_exp_pred r).
+    glu_sort_elem_econstructor; eauto; reflexivity.
+
+  - saturate_refl.
     do 2 eexists.
     glu_sort_elem_econstructor; eauto; reflexivity.
 Qed.
@@ -1190,7 +1123,28 @@ Ltac saturate_glu_info :=
 #[local]
 Hint Rewrite -> @sub_decompose_q using solve [mauto 4] : mcpts.
 
-  
+Lemma glu_nat_monotone {P} {s} (r : Ru_nat P s) : forall Γ M m,
+    {{ ⊢ Γ }} ->
+    glu_nat r Γ M m ->
+    forall Δ σ,
+      {{ Δ ⊢w σ : Γ }} ->
+      glu_nat r Δ {{{ M[σ] }}} m.
+Proof.
+  intros * HΓ Hglu.
+  assert {{ Γ ⊢ M : ℕ }} by mauto 2.
+  induction Hglu; intros; econstructor; mauto 2.
+  - transitivity {{{ zero[σ] }}}; mauto 3.
+  - transitivity {{{ (succ M')[σ] }}}; mauto 3.
+    econstructor; mauto 3.
+  - eapply IHHglu; mauto 3.
+  - intros.
+    assert {{ Δ0 ⊢w σ∘σ0 : Γ }} by mauto.
+    assert {{ Δ0 ⊢ M[σ∘σ0] ≈ M' : ℕ }} by mauto 3.
+    transitivity {{{ M[σ∘σ0] }}}; mauto 3.
+    eapply (@exp_eq_sub_compose_nat P Δ0 Γ Δ M σ σ0 s r); mauto 2.
+Qed.
+    
+    
 Lemma glu_sort_elem_mut_monotone {P} (pred_P : PredicativeSig P) : forall s a typ_rel exp_rel,
     {{ DG a ∈ glu_sort_elem pred_P s ↘ typ_rel ↘ exp_rel }} ->
     forall Δ σ Γ,
@@ -1209,79 +1163,12 @@ Proof.
     simpl in *;
     destruct_all;
     try solve [bulky_rewrite].
-  - transitivity {{{ Sort@s'[σ] }}}; mauto 2.
-    (* repeat split; intros; [transitivity {{{ Sort@s'[σ] }}}; mauto 2 | |]; *)
-    (*   assert {{ Δ0 ⊢w σ∘σ0 : Γ }} by mauto 2.       *)
-    (* + gen_presup H0. *)
-    (*   assert {{ Δ0 ⊢ A[σ∘σ0] ≈ A[σ][σ0] }} by mauto 3. *)
-    (*   assert {{ Δ0 ⊢ A[σ∘σ0] ≈ A[σ][σ0] : K }} by (eapply H1; mauto 3). *)
-    (*   gen_presup H9. *)
-    (*   assert {{ Δ0 ⊢ A[σ∘σ0] ≈ A' }} by (transitivity {{{ A[σ][σ0] }}}; mauto 3). *)
-    (*   assert ({{ Δ0 ⊢ A[σ∘σ0] : K }} -> {{ Δ0 ⊢ A[σ∘σ0] ≈ A' : K }}) by (eapply H1; mauto 3). *)
-    (*   transitivity {{{ A[σ∘σ0] }}}; mauto 3. *)
-    (* + gen_presup H0. *)
-    (*   assert {{ Δ0 ⊢ A[σ∘σ0] ≈ A[σ][σ0] }} by mauto 3. *)
-    (*   assert {{ Δ0 ⊢ A[σ∘σ0] ≈ A' }} by (transitivity {{{ A[σ][σ0] }}}; mauto 3). *)
-    (*   assert {{ Δ0 ⊢ A[σ∘σ0] ≈ A' : K }} by (eapply H1; mauto 3). *)
-    (*   gen_presup H10. *)
-    (*   assert ({{ Δ0 ⊢ A[σ∘σ0] : K }} -> {{ Δ0 ⊢ A[σ∘σ0] ≈ A[σ][σ0] : K }}) by (eapply H1; mauto 3). *)
-    (*   transitivity {{{ A[σ∘σ0] }}}; mauto 3. *)
-      
-  - repeat split; intros; mauto 4.
-    (* + gen_presup H0. *)
-    (*   assert {{ Δ0 ⊢ A[σ∘σ0] ≈ A[σ][σ0] }} by mauto 3. *)
-    (*   assert {{ Δ0 ⊢ A[σ∘σ0] ≈ A[σ][σ0] : K }} by (eapply H3; mauto 3). *)
-    (*   gen_presup H11. *)
-    (*   assert {{ Δ0 ⊢ A[σ∘σ0] ≈ A' }} by (transitivity {{{ A[σ][σ0] }}}; mauto 3). *)
-    (*   assert ({{ Δ0 ⊢ A[σ∘σ0] : K }} -> {{ Δ0 ⊢ A[σ∘σ0] ≈ A' : K }}) by (eapply H3; mauto 3). *)
-    (*   transitivity {{{ A[σ∘σ0] }}}; mauto 3. *)
-    (* + gen_presup H0. *)
-    (*   assert {{ Δ0 ⊢ A[σ∘σ0] ≈ A[σ][σ0] }} by mauto 3. *)
-    (*   assert {{ Δ0 ⊢ A[σ∘σ0] ≈ A' }} by (transitivity {{{ A[σ][σ0] }}}; mauto 3). *)
-    (*   assert {{ Δ0 ⊢ A[σ∘σ0] ≈ A' : K }} by (eapply H3; mauto 3). *)
-    (*   gen_presup H12. *)
-    (*   assert ({{ Δ0 ⊢ A[σ∘σ0] : K }} -> {{ Δ0 ⊢ A[σ∘σ0] ≈ A[σ][σ0] : K }}) by (eapply H3; mauto 3). *)
-    (*   transitivity {{{ A[σ∘σ0] }}}; mauto 3. *)
-    (* + assert {{ Γ ⊢ M }} by mauto 3. *)
-    (*   assert {{ Δ0 ⊢ M[σ∘σ0] ≈ M[σ][σ0] }} by mauto 3. *)
-    (*   assert {{ Δ0 ⊢ M[σ∘σ0] ≈ M[σ][σ0] : B }} by (eapply H5; mauto 3). *)
-    (*   gen_presup H13. *)
-    (*   assert {{ Δ0 ⊢ M[σ∘σ0] ≈ M' }} by (transitivity {{{ M[σ][σ0] }}}; mauto 3). *)
-    (*   assert ({{ Δ0 ⊢ M[σ∘σ0] : B }} -> {{ Δ0 ⊢ M[σ∘σ0] ≈ M' : B }}) by (eapply H5; mauto 3). *)
-    (*   transitivity {{{ M[σ∘σ0] }}}; mauto 3. *)
-    (* + assert {{ Γ ⊢ M }} by mauto 3. *)
-    (*   assert {{ Δ0 ⊢ M[σ∘σ0] ≈ M[σ][σ0] }} by mauto 3. *)
-    (*   assert {{ Δ0 ⊢ M[σ∘σ0] ≈ M' : B }} by (eapply H5; mauto 3). *)
-    (*   gen_presup H13. *)
-    (*   assert {{ Δ0 ⊢ M[σ∘σ0] ≈ M' }} by (transitivity {{{ M[σ][σ0] }}}; mauto 3). *)
-    (*   assert ({{ Δ0 ⊢ M[σ∘σ0] : B }} -> {{ Δ0 ⊢ M[σ∘σ0] ≈ M[σ][σ0] : B }}) by (eapply H5; mauto 3). *)
-    (*   transitivity {{{ M[σ∘σ0] }}}; mauto 3. *)
-    + repeat eexists; mauto 2; bulky_rewrite.
-      resp_per_IH.
 
+  - repeat eexists; mauto 2; bulky_rewrite.
+    resp_per_IH.
   - destruct H7.
     simpl_glu_rel.
-    assert ({{ Γ ⊢ IT : Sort@s1 }} /\ {{ Γ, IT ⊢ OT : Sort@s2 }}) by (gen_presup H4; mauto 3).
-    destruct_conjs.
-    assert {{ Δ ⊢ (Π r IT OT)[σ] ≈ Π r IT[σ] OT[q σ] }} by mauto 3.
-    assert {{ Δ ⊢ A[σ] ≈ Π r IT[σ] OT[q σ] }} by (transitivity {{{ (Π r IT OT)[σ] }}}; mauto 4).
-    
-    econstructor; eauto; try solve [bulky_rewrite]; mauto 4.
-    (* + repeat split; intros. *)
-    (*   * assert {{ Γ ⊢ A }} by mauto 2. *)
-    (*     assert {{ Δ0 ⊢ A[σ∘σ0] ≈ A[σ][σ0] }} by mauto 3. *)
-    (*     assert {{ Δ0 ⊢ A[σ∘σ0] ≈ A[σ][σ0] : K }} by (eapply H9; mauto 3). *)
-    (*     gen_presup H17. *)
-    (*     assert {{ Δ0 ⊢ A[σ∘σ0] ≈ A' }} by (transitivity {{{ A[σ][σ0] }}}; mauto 3). *)
-    (*     assert ({{ Δ0 ⊢ A[σ∘σ0] : K }} -> {{ Δ0 ⊢ A[σ∘σ0] ≈ A' : K }}) by (eapply H9; mauto 3). *)
-    (*     transitivity {{{ A[σ∘σ0] }}}; mauto 3. *)
-    (*   * assert {{ Γ ⊢ A }} by mauto 2. *)
-    (*     assert {{ Δ0 ⊢ A[σ∘σ0] ≈ A[σ][σ0] }} by mauto 3. *)
-    (*     assert {{ Δ0 ⊢ A[σ∘σ0] ≈ A' }} by (transitivity {{{ A[σ][σ0] }}}; mauto 3). *)
-    (*     assert {{ Δ0 ⊢ A[σ∘σ0] ≈ A' : K }} by (eapply H9; mauto 3). *)
-    (*     gen_presup H18. *)
-    (*     assert ({{ Δ0 ⊢ A[σ∘σ0] : K }} -> {{ Δ0 ⊢ A[σ∘σ0] ≈ A[σ][σ0] : K }}) by (eapply H9; mauto 3). *)
-    (*     transitivity {{{ A[σ∘σ0] }}}; mauto 3.       *)
+    econstructor; eauto; try solve [bulky_rewrite]; mauto 3.
     + intros.
       eapply IHglu_sort_elem; eauto.
     + intros.
@@ -1293,49 +1180,22 @@ Proof.
       deepexec H1 ltac:(fun H => pose proof H).
       assert {{ Δ0 ⊢s (q σ)∘(σ0,,M) ≈ σ∘σ0,,M : Γ, IT }} by mauto.
       assert {{ Δ, IT[σ] ⊢s q σ : Γ, IT }} by mauto 3.
-      assert {{ Δ0 ⊢s σ0,,M : Δ, IT[σ] }} by mauto 4.
+      assert {{ Δ0 ⊢s σ0,,M : Δ, IT[σ] }} by mauto 3.
       assert {{ Δ0 ⊢ OT[(q σ)∘(σ0,,M)] ≈ OT[q σ][σ0,,M] : Sort@s2[(q σ)∘(σ0,,M)] }} by mauto.
       assert {{ Δ0 ⊢ OT[q σ][σ0,,M] ≈ OT[(q σ)∘(σ0,,M)] : Sort@s2 }} by mauto.
-      assert {{ Δ0 ⊢ OT[(q σ)∘(σ0,,M)] ≈ OT[q σ][σ0,,M] : Sort@s2[(q σ)∘(σ0,,M)] }} by mauto.
-      assert {{ Δ0 ⊢ OT[q σ][σ0,,M] ≈ OT[(q σ)∘(σ0,,M)] : Sort@s2 }} by mauto.
-      assert {{ Δ0 ⊢ OT[(q σ)∘(σ0,,M)] ≈ OT[σ∘σ0,,M] : Sort@s2[(q σ)∘(σ0,,M)] }} by mauto.
-      assert {{ Δ0 ⊢ OT[(q σ)∘(σ0,,M)] ≈ OT[σ∘σ0,,M] : Sort@s2 }} by mauto 4.
       assert {{ Δ0 ⊢ OT[q σ][σ0,,M] ≈ OT[σ∘σ0,,M] : Sort@s2 }} by mauto.
-      
-      enough (OP m equiv_m Δ0 {{{ OT[σ∘σ0,,M] }}}) by (eapply glu_sort_elem_typ_resp_typ_eq; mauto 3).
+      enough (OP m equiv_m Δ0 {{{ OT[σ∘σ0,,M] }}}) by (eapply glu_sort_elem_typ_resp_exp_eq; mauto 2).
       eapply H10; mauto.
       assert {{ Δ0 ⊢ IT[σ∘σ0] ≈ IT[σ][σ0] : Sort@s1[σ∘σ0] }} by mauto.
       assert {{ Δ0 ⊢ IT[σ∘σ0] ≈ IT[σ][σ0] : Sort@s1 }} by mauto 4.
-      
-      enough (IEL Δ0 {{{ IT[σ][σ0] }}} M m) by (eapply glu_sort_elem_trm_resp_typ_eq; mauto).
+      enough (IEL Δ0 {{{ IT[σ][σ0] }}} M m) by (eapply glu_sort_elem_trm_resp_typ_exp_eq; mauto).
       eassumption.
-      
+
   - destruct H7.
     simpl_glu_rel.
-    assert ({{ Γ ⊢ IT : Sort@s1 }} /\ {{ Γ, IT ⊢ OT : Sort@s2 }}) by (gen_presup H7; mauto 3).
-    destruct_conjs.
-    assert {{ Δ ⊢ (Π r IT OT)[σ] ≈ Π r IT[σ] OT[q σ] }} by mauto 3.
-    assert {{ Δ ⊢ A[σ] ≈ Π r IT[σ] OT[q σ] }} by (transitivity {{{ (Π r IT OT)[σ] }}}; mauto 4).
-    
     econstructor; mauto 4;
       intros;
       saturate_weakening_escape.
-    (* + split; intros. *)
-    (*   * assert {{ Γ ⊢ A }} by mauto 2. *)
-    (*     assert {{ Δ0 ⊢ A[σ∘σ0] ≈ A[σ][σ0] }} by mauto 3. *)
-    (*     assert {{ Δ0 ⊢ A[σ∘σ0] ≈ A[σ][σ0] : K }} by (eapply H11; mauto 3). *)
-    (*     gen_presup H20. *)
-    (*     assert {{ Δ0 ⊢ A[σ∘σ0] ≈ A' }} by (transitivity {{{ A[σ][σ0] }}}; mauto 3). *)
-    (*     assert ({{ Δ0 ⊢ A[σ∘σ0] : K }} -> {{ Δ0 ⊢ A[σ∘σ0] ≈ A' : K }}) by (eapply H11; mauto 3). *)
-    (*     transitivity {{{ A[σ∘σ0] }}}; mauto 3. *)
-    (*   * assert {{ Γ ⊢ A }} by mauto 2. *)
-    (*     assert {{ Δ0 ⊢ A[σ∘σ0] ≈ A[σ][σ0] }} by mauto 3. *)
-    (*     assert {{ Δ0 ⊢ A[σ∘σ0] ≈ A' }} by (transitivity {{{ A[σ][σ0] }}}; mauto 3). *)
-    (*     assert {{ Δ0 ⊢ A[σ∘σ0] ≈ A' : K }} by (eapply H11; mauto 3). *)
-    (*     gen_presup H21. *)
-    (*     assert ({{ Δ0 ⊢ A[σ∘σ0] : K }} -> {{ Δ0 ⊢ A[σ∘σ0] ≈ A[σ][σ0] : K }}) by (eapply H11; mauto 3). *)
-    (*     transitivity {{{ A[σ∘σ0] }}}; mauto 3. *)
-        
     + eapply IHglu_sort_elem; eauto.
     + saturate_glu_info.
       invert_per_sort_elem H3.
@@ -1346,92 +1206,93 @@ Proof.
       deepexec H1 ltac:(fun H => pose proof H).
       autorewrite with mcpts in *.
       repeat eexists; eauto.
-      assert {{ Δ0 ⊢s σ0,,N : Δ, IT[σ] }} by mauto 4.
+      assert {{ Δ0 ⊢s σ0,,N : Δ, IT[σ] }} by mauto 3.
       assert {{ Γ ⊢ M : Π r IT OT }} by mauto.
       assert {{ Δ0 ⊢ M[σ][σ0] : (Π r IT OT)[σ][σ0] }} by mauto.
       assert {{ Δ0 ⊢ (Π r IT OT)[σ][σ0] ≈ (Π r IT OT)[σ∘σ0] }} by (symmetry; mauto 3).
       assert {{ Δ0 ⊢ M[σ][σ0] ≈ M[σ∘σ0] : (Π r IT OT)[σ][σ0] }} by mauto.
-      assert {{ Δ0 ⊢ (Π r IT OT)[σ∘σ0] ≈ Π r IT[σ∘σ0] OT[q (σ∘σ0)] }} by mauto.
+      assert {{ Δ0 ⊢ (Π r IT OT)[σ∘σ0] ≈ Π r IT[σ∘σ0] OT[q (σ∘σ0)] }} by mauto 4.
       assert {{ Δ0 ⊢ M[σ][σ0] ≈ M[σ∘σ0] : Π r IT[σ∘σ0] OT[q (σ∘σ0)] }} by mauto.
       assert {{ Δ0 ⊢ IT[σ∘σ0] : Sort@s1 }} by mauto.
       assert {{ Δ0 ⊢ IT[σ∘σ0] ≈ IT[σ][σ0] }} by mauto.
-      assert {{ Δ0, IT[σ∘σ0] ⊢ #0 : IT[(σ∘σ0)][Wk] }} by (do 2 (econstructor; mauto 2)).
+      assert {{ Δ0, IT[σ∘σ0] ⊢ #0 : IT[(σ∘σ0)][Wk] }} by (do 2 econstructor; mauto 2).
       assert {{ Δ0, IT[σ∘σ0] ⊢ IT[(σ∘σ0)∘Wk] ≈ IT[σ∘σ0][Wk] }} by (eapply wf_typ_eq_sub_compose; mauto 3).
       assert {{ Δ0, IT[σ∘σ0] ⊢ #0 : IT[(σ∘σ0)∘Wk] }} by mauto 3.
       assert {{ Δ0, IT[σ∘σ0] ⊢ OT[q (σ∘σ0)] : Sort@s2[q (σ∘σ0)] }} by (repeat (econstructor; mauto 2)).
-      assert {{ Δ0, IT[σ∘σ0] ⊢ Sort@s2 ≈ Sort@s2[q (σ∘σ0)] }} by (symmetry; econstructor; mauto 4).
+      assert {{ Δ0, IT[σ∘σ0] ⊢ Sort@s2 ≈ Sort@s2[q (σ∘σ0)] }} by mauto.
       assert {{ Δ0, IT[σ∘σ0] ⊢ OT[q (σ∘σ0)] : Sort@s2 }} by mauto.
-      
       assert {{ Δ0 ⊢ M[σ][σ0] N ≈ M[σ∘σ0] N : OT[q (σ∘σ0)][Id,,N] }}.
       {
         eapply wf_exp_eq_app_cong; mauto 2.
         econstructor; mauto 2.
       }
-      
-      assert {{ Δ0 ⊢ OT[(q (σ∘σ0))∘(Id,,N)] ≈ OT[q (σ∘σ0)][Id,,N] }} by (eapply wf_typ_eq_sub_compose; mauto).
+      assert {{ Δ0 ⊢ OT[(q (σ∘σ0))∘(Id,,N)] ≈ OT[q (σ∘σ0)][Id,,N] }} by (eapply wf_typ_eq_sub_compose; mauto 4).
       assert {{ Δ0 ⊢s (q (σ∘σ0))∘(Id,,N) ≈ σ∘σ0,,N : Γ, IT }}.
       {
         eapply sub_eq_q_sigma_id_extend; mauto 2.
         econstructor; mauto 2.
       }
-      (* assert {{ Δ0 ⊢ OT[(q (σ∘σ0))∘(Id,,N)] ≈ OT[σ∘σ0,,N] : Sort@s2 }} by mauto. *)
+      assert {{ Γ, IT ⊢ OT ≈ OT : Sort@s2 }} by mauto 3.
+      assert {{ Δ0 ⊢ OT[(q (σ∘σ0))∘(Id,,N)] ≈ OT[σ∘σ0,,N] : Sort@s2 }}.
+      {
+        gen_presup H40.
+        eapply eq_exp_eq_sub_typ; mauto 2.        
+      }
       assert {{ Δ0 ⊢ OT[(q (σ∘σ0))∘(Id,,N)] ≈ OT[σ∘σ0,,N] }} by mauto.
       assert {{ Δ0 ⊢ OT[q (σ∘σ0)][Id,,N] ≈ OT[σ∘σ0,,N] }} by mauto.
       assert {{ Δ0 ⊢ M[σ][σ0] N ≈ M[σ∘σ0] N : OT[σ∘σ0,,N] }} by mauto.
-
-
       assert {{ Δ0 ⊢s (q σ)∘(σ0,,N) ≈ (σ∘σ0),,N : Γ, IT }} by (eapply sub_eq_q_sigma_sigma0_extend; mauto 2).
-      
-      assert {{ Δ0 ⊢ OT[(q σ)∘(σ0,,N)] ≈ OT[q σ][σ0,,N] : Sort@s2[(q σ)∘(σ0,,N)] }} by mauto 4.
-      assert {{ Δ0 ⊢ Sort@s2[(q σ)∘(σ0,,N)] ≈ Sort@s2 }} by mauto.
+      assert {{ Δ0 ⊢ OT[(q σ)∘(σ0,,N)] ≈ OT[q σ][σ0,,N] : Sort@s2[(q σ)∘(σ0,,N)] }} by mauto.
       assert {{ Δ0 ⊢ OT[(q σ)∘(σ0,,N)] ≈ OT[q σ][σ0,,N] : Sort@s2 }} by mauto.
       assert {{ Δ0 ⊢ OT[(q σ)∘(σ0,,N)] ≈ OT[σ∘σ0,,N] : Sort@s2 }} by mauto 4.
       assert {{ Δ0 ⊢ OT[q σ][σ0,,N] ≈ OT[σ∘σ0,,N] : Sort@s2 }} by mauto.
-      enough (OEL n equiv_n Δ0 {{{ OT[σ∘σ0,,N] }}} {{{ M[σ][σ0] N }}} fa) by (eapply glu_sort_elem_trm_resp_typ_eq; mauto 3).
+      enough (OEL n equiv_n Δ0 {{{ OT[σ∘σ0,,N] }}} {{{ M[σ][σ0] N }}} fa) by (eapply glu_sort_elem_trm_resp_typ_exp_eq; mauto 3).
       enough (OEL n equiv_n Δ0 {{{ OT[σ∘σ0,,N] }}} {{{ M[σ∘σ0] N }}} fa) by (eapply glu_sort_elem_trm_resp_exp_eq; mauto 3).
-
-      assert (exists mn : domain P, {{ $| m & n |↘ mn }} /\ OEL n equiv_n Δ0 {{{ OT[σ∘σ0,,N] }}} {{{ M[σ∘σ0] N }}} mn) by mauto 3.
+      assert (exists mn : domain P, {{ $| m & n |↘ mn }} /\ OEL n equiv_n Δ0 {{{ OT[σ∘σ0,,N] }}} {{{ M[σ∘σ0] N }}} mn).
+      {
+        eapply H12; mauto.
+        enough (IEL Δ0 {{{ IT[σ][σ0] }}} N n).
+        {
+          eapply glu_sort_elem_trm_resp_typ_exp_eq; mauto 3.
+          symmetry.
+          econstructor; mauto 3.
+        }
+        eassumption.
+      }
       destruct_conjs.
       simplify_evals.
       eassumption.
-      
-  - split; [mauto 3 |].
-    repeat split; intros.
-    (* + assert {{ Γ ⊢ A }} by mauto 2. *)
-    (*   assert {{ Δ0 ⊢ A[σ∘σ0] ≈ A[σ][σ0] }} by mauto 3. *)
-    (*   assert {{ Δ0 ⊢ A[σ∘σ0] ≈ A[σ][σ0] : K }} by (eapply H1; mauto 3). *)
-    (*   gen_presup H10. *)
-    (*   assert {{ Δ0 ⊢ A[σ∘σ0] ≈ A' }} by (transitivity {{{ A[σ][σ0] }}}; mauto 3). *)
-    (*   assert ({{ Δ0 ⊢ A[σ∘σ0] : K }} -> {{ Δ0 ⊢ A[σ∘σ0] ≈ A' : K }}) by (eapply H1; mauto 3). *)
-    (*   transitivity {{{ A[σ∘σ0] }}}; mauto 3. *)
-    (* + assert {{ Γ ⊢ A }} by mauto 2. *)
-    (*   assert {{ Δ0 ⊢ A[σ∘σ0] ≈ A[σ][σ0] }} by mauto 3. *)
-    (*   assert {{ Δ0 ⊢ A[σ∘σ0] ≈ A' }} by (transitivity {{{ A[σ][σ0] }}}; mauto 3). *)
-    (*   assert {{ Δ0 ⊢ A[σ∘σ0] ≈ A' : K }} by (eapply H1; mauto 3). *)
-    (*   gen_presup H11. *)
-    (*   assert ({{ Δ0 ⊢ A[σ∘σ0] : K }} -> {{ Δ0 ⊢ A[σ∘σ0] ≈ A[σ][σ0] : K }}) by (eapply H1; mauto 3). *)
-    (*   transitivity {{{ A[σ∘σ0] }}}; mauto 3. *)
-    + intros; mauto 3.
-      transitivity {{{ A[σ∘σ0] }}}; mauto 4.
-    
+
+  - destruct_conjs.
+    split; [mauto 3 |].
+    intros.
+    saturate_weakening_escape.
+    transitivity {{{ A[σ∘σ0] }}}.
+    + symmetry.
+      mauto.
+    + eapply H1; mauto.
+
   - simpl_glu_rel.
     econstructor; repeat split; mauto 3;
       intros;
       saturate_weakening_escape.
-    (* + assert {{ Δ0 ⊢ A[σ∘σ0] ≈ A[σ][σ0] }} by mauto 3. *)
-    (*   assert {{ Δ0 ⊢ A[σ∘σ0] ≈ A[σ][σ0] : K }} by (eapply H1; mauto 3). *)
-    (*   gen_presup H13. *)
-    (*   assert {{ Δ0 ⊢ A[σ∘σ0] ≈ A' }} by (transitivity {{{ A[σ][σ0] }}}; mauto 3). *)
-    (*   assert ({{ Δ0 ⊢ A[σ∘σ0] : K }} -> {{ Δ0 ⊢ A[σ∘σ0] ≈ A' : K }}) by (eapply H1; mauto 3). *)
-    (*   transitivity {{{ A[σ∘σ0] }}}; mauto 3. *)
-    (* + assert {{ Δ0 ⊢ A[σ∘σ0] ≈ A[σ][σ0] }} by mauto 3. *)
-    (*   assert {{ Δ0 ⊢ A[σ∘σ0] ≈ A' }} by (transitivity {{{ A[σ][σ0] }}}; mauto 3). *)
-    (*   assert {{ Δ0 ⊢ A[σ∘σ0] ≈ A' : K }} by (eapply H1; mauto 3). *)
-    (*   gen_presup H14. *)
-    (*   assert ({{ Δ0 ⊢ A[σ∘σ0] : K }} -> {{ Δ0 ⊢ A[σ∘σ0] ≈ A[σ][σ0] : K }}) by (eapply H1; mauto 3). *)
-    (*   transitivity {{{ A[σ∘σ0] }}}; mauto 3.     *)
-    + transitivity {{{ A[σ∘σ0] }}}; mauto 4.      
-    + transitivity {{{ M[σ∘σ0] }}}; [symmetry|]; mauto 5.
+    + transitivity {{{ A[σ∘σ0] }}}.
+      * symmetry.
+        mauto.
+      * eapply H1; mauto.
+    + transitivity {{{ M[σ∘σ0] }}}.
+      * symmetry; mauto.
+      * enough {{ Δ0 ⊢ M[σ∘σ0] ≈ M' : A[σ∘σ0] }} by mauto.
+        eapply H5; mauto.
+
+  - transitivity {{{ ℕ[σ] }}}; mauto 4.
+    econstructor; mauto.
+
+  - split. 
+    + transitivity {{{ ℕ[σ] }}}; mauto 4.
+      econstructor; mauto.
+    + gen_presup H3.
+      eapply glu_nat_monotone; mauto 2.
 Qed.
 
 
@@ -1456,6 +1317,8 @@ Proof.
   eapply glu_sort_elem_mut_monotone in H; eauto.
   intuition.
 Qed.
+
+(* STOPPED HERE *)
 
 Add Parametric Morphism {P} (pred_P : PredicativeSig P) (s : P) a : (glu_elem_bot pred_P s a)
     with signature wf_ctx_eq ==> eq ==> eq ==> eq ==> iff as glu_elem_bot_morphism_iff1.
